src/dvspec/dafny/implementation/dvc_implementation.dfy
@@ -1,39 +1,34 @@
 include "../commons.dfy"
+
 abstract module DVCNode_Implementation
 {
     import opened Types
     import opened CommonFunctions
-    import opened DVCNode_Externs: DVCNode_Externs
+    import opened DVCNode_Externs : DVCNode_Externs
 
     export PublicInterface
-        reveals DVCNode,
-                AttestationSignatureShareDB
+        reveals DVCNode        
         provides
-                DVCNode.serve_attestation_duty, 
-                DVCNode.att_consensus_decided, 
-                DVCNode.listen_for_attestation_shares,
-                DVCNode.listen_for_new_imported_blocks,
-                DVCNode.resend_attestation_share,
-                DVCNode.bn
+                DVCNode.process_event,
+                DVCNode.getRepr,
+                DVCNode.ValidConstructorRepr,
+                DVCNode.ValidRepr
         provides Types, DVCNode_Externs
-
-    type AttestationSignatureShareDB = map<(AttestationData, seq<bool>), set<AttestationShare>>   
 
     class DVCNode {
 
         var current_attesation_duty: Optional<AttestationDuty>;
+        var latest_attestation_duty: Optional<AttestationDuty>;
         var attestation_duties_queue: seq<AttestationDuty>;
-        // var pubkey: BLSPubkey;
-        var attestation_slashing_db: AttestationSlashingDB;
-        var attestation_shares_db: AttestationSignatureShareDB;
-        var attestation_share_to_broadcast: Optional<AttestationShare>
+        var rcvd_attestation_shares: map<Slot,map<(AttestationData, seq<bool>), set<AttestationShare>>>;
+        var attestation_shares_to_broadcast: map<Slot, AttestationShare>
         var construct_signed_attestation_signature: (set<AttestationShare>) -> Optional<BLSSignature>;
         var peers: set<BLSPubkey>;
-        // TODO: Note difference with spec.py
         var dv_pubkey: BLSPubkey;
-        var future_att_consensus_instances_already_decided: set<Slot>
+        var future_att_consensus_instances_already_decided: map<Slot, AttestationData>
 
-        var att_consensus: Consensus;
+        const slashing_db: SlashingDB;
+        const att_consensus: Consensus<AttestationData>;
         const network : Network
         const bn: BeaconNode;
         const rs: RemoteSigner;
@@ -41,105 +36,162 @@ abstract module DVCNode_Implementation
         constructor(
             pubkey: BLSPubkey, 
             dv_pubkey: BLSPubkey,
-            att_consensus: Consensus, 
+            att_consensus: Consensus<AttestationData>, 
             peers: set<BLSPubkey>,
             network: Network,
             bn: BeaconNode,
             rs: RemoteSigner,
-            construct_signed_attestation_signature: (set<AttestationShare>) -> Optional<BLSSignature>)
+            initial_slashing_db: SlashingDB,
+            construct_signed_attestation_signature: (set<AttestationShare>) -> Optional<BLSSignature>
+        )
+        // The following indicates that `att_consensus` must not have any active consensus instance running.
+        // This may need to be strengthened to require that `att_consensus` has never started any consensus instance.
+        requires att_consensus.consensus_instances_started == map[]
+        requires ValidConstructorRepr(att_consensus, network, bn, rs, initial_slashing_db)
         {
             current_attesation_duty := None;
-            attestation_share_to_broadcast := None;
-            attestation_shares_db := map[];
+            latest_attestation_duty := None;
+            attestation_duties_queue := [];
+            slashing_db := initial_slashing_db;
+            attestation_shares_to_broadcast := map[];
+            rcvd_attestation_shares := map[];
+            future_att_consensus_instances_already_decided := map[];
 
-            // this.pubkey := pubkey;
             this.att_consensus := att_consensus;
             this.peers := peers;
             this.network := network;
             this.rs := rs;
             this.bn := bn;
             this.construct_signed_attestation_signature := construct_signed_attestation_signature;
-            this.dv_pubkey := dv_pubkey;
-            this.future_att_consensus_instances_already_decided := {};
+            this.dv_pubkey := dv_pubkey;        
         }
+    
+        /*=================================================================================
+         * Public methods
+         * ===============================================================================*/
+
+        method process_event(
+            event: Event
+        ) returns (s: Status)
+        requires ValidRepr()
+        modifies getRepr()
+        {
+            match event {
+                case ServeAttstationDuty(attestation_duty) => 
+                    :- serve_attestation_duty(attestation_duty);
+                case AttConsensusDecided(id, decided_attestation_data) => 
+                    :- att_consensus_decided(id,  decided_attestation_data);
+                case ReceviedAttesttionShare(attestation_share) => 
+                    listen_for_attestation_shares(attestation_share);
+                case ImportedNewBlock(block) => 
+                    :- listen_for_new_imported_blocks(block);
+                case ResendAttestationShares => 
+                    resend_attestation_share();
+                case NoEvent =>
+                    
+            }
+
+            {return Success;}
+        }   
+        
+        /*=================================================================================
+         * Private methods
+         * ===============================================================================*/        
 
         method serve_attestation_duty(
             attestation_duty: AttestationDuty
-        )
-        modifies this
+        ) returns (s: Status)
+        requires ValidRepr()
+        modifies getRepr()
         {
             attestation_duties_queue := attestation_duties_queue + [attestation_duty];
-            check_for_next_queued_duty();
+            { :- check_for_next_queued_duty();}
+
+            return Success;
         }
 
-        method check_for_next_queued_duty()
-        modifies this
+        method check_for_next_queued_duty() returns (s: Status) // TODO T/O
+        requires ValidRepr()
+        modifies getRepr()
         decreases attestation_duties_queue
         {
             if attestation_duties_queue != []
             {
-                if attestation_duties_queue[0].slot in future_att_consensus_instances_already_decided
+                if attestation_duties_queue[0].slot in future_att_consensus_instances_already_decided.Keys
                 {
+                    var queue_head := attestation_duties_queue[0];
                     attestation_duties_queue := attestation_duties_queue[1..];
-                    check_for_next_queued_duty();
+                    update_attestation_slashing_db(future_att_consensus_instances_already_decided[queue_head.slot]);
+                    future_att_consensus_instances_already_decided := future_att_consensus_instances_already_decided - {queue_head.slot};                    
+                    { :- check_for_next_queued_duty();}
                 }
-                else
+                else if !current_attesation_duty.isPresent()
                 {
-                    start_next_duty(attestation_duties_queue[0]);
+                    var queue_head := attestation_duties_queue[0];
+                    attestation_duties_queue := attestation_duties_queue[1..];
+
+                    :- start_next_duty(queue_head);
                 }
             }
+
+            return Success;
         }
 
-        method start_next_duty(attestation_duty: AttestationDuty)
-        modifies this
+        method start_next_duty(attestation_duty: AttestationDuty) returns (s: Status)
+        requires ValidRepr()
+        modifies getRepr()
         {
-            attestation_shares_db := map[];
-            attestation_share_to_broadcast := None;
             current_attesation_duty := Some(attestation_duty);
-            att_consensus.start(attestation_duty.slot);            
+            latest_attestation_duty := Some(attestation_duty);
+            var validityCheck := new AttestationConsensusValidityCheck(this.dv_pubkey, this.slashing_db, attestation_duty);
+            { :- att_consensus.start(attestation_duty.slot, validityCheck);}
+            return Success;
         }        
 
-        method update_attestation_slashing_db(attestation_data: AttestationData, attestation_duty_pubkey: BLSPubkey)
-        modifies this       
+        method update_attestation_slashing_db(attestation_data: AttestationData)
+        requires ValidRepr()
+        modifies slashing_db.Repr
+        ensures fresh(slashing_db.Repr - old(slashing_db.Repr))
+        ensures  ValidRepr()
         {
-            // assert not is_slashable_attestation_data(attestation_slashing_db, attestation_data, pubkey)
-            // TODO: Is the following required given that each co-validator only handles one pubkey?
-            // slashing_db_data = get_slashing_db_data_for_pubkey(attestation_slashing_db, pubkey)
             var slashing_db_attestation := SlashingDBAttestation(
                                                 source_epoch := attestation_data.source.epoch,
                                                 target_epoch := attestation_data.target.epoch,
-                                                signing_root := hash_tree_root(attestation_data));
-            attestation_slashing_db := attestation_slashing_db + {slashing_db_attestation};
+                                                signing_root := Some(hash_tree_root(attestation_data)));
+            slashing_db.add_attestation(slashing_db_attestation, dv_pubkey);
         }
 
         method att_consensus_decided(
             id: Slot,
             decided_attestation_data: AttestationData
         ) returns (r: Status)
-        modifies this
+        requires ValidRepr()
+        modifies getRepr()
         {
-            var local_current_attestation_duty :- current_attesation_duty.get();
-            update_attestation_slashing_db(decided_attestation_data, local_current_attestation_duty.pubkey);
+            var local_current_attestation_duty :- current_attesation_duty.get();            
+            update_attestation_slashing_db(decided_attestation_data);
  
             var fork_version := bn.get_fork_version(compute_start_slot_at_epoch(decided_attestation_data.target.epoch));
             var attestation_signing_root := compute_attestation_signing_root(decided_attestation_data, fork_version);
             var attestation_signature_share := rs.sign_attestation(decided_attestation_data, fork_version, attestation_signing_root);
-            // TODO: What is attestation_signature_share.aggregation_bits?
             var attestation_with_signature_share := AttestationShare(
                 aggregation_bits := get_aggregation_bits(local_current_attestation_duty.validator_index),
                 data := decided_attestation_data, 
                 signature :=attestation_signature_share
             ); 
 
-            attestation_share_to_broadcast := Some(attestation_with_signature_share);
-            network.send_att_share(attestation_with_signature_share, peers);           
+            attestation_shares_to_broadcast := attestation_shares_to_broadcast[local_current_attestation_duty.slot := attestation_with_signature_share];
+            network.send_att_share(attestation_with_signature_share, peers);  
+            current_attesation_duty := None;
+            
+            { :- check_for_next_queued_duty(); }
+
+            return Success;         
         }
 
         function method get_aggregation_bits(
             index: nat
-        ): (s: seq<bool>)
-        ensures |s| == index
-        ensures forall i | 0 <= i < |s| :: if i == index - 1 then s[i] else !s[i]
+        ): seq<bool>
         {
             seq(index, i => if i + 1 == index then true else false)
         }        
@@ -147,79 +199,195 @@ abstract module DVCNode_Implementation
         method listen_for_attestation_shares(
             attestation_share: AttestationShare
         )
-        modifies this
+        requires ValidRepr()
+        modifies getRepr()
         {
-            // TODO: Decide 
-            // 1. whether to add att shares to db only if already served attestation duty
-            // 2. when to wipe out the db
-            var k := (attestation_share.data, attestation_share.aggregation_bits);
-            attestation_shares_db := 
-                attestation_shares_db[k := 
-                                        getOrDefault(attestation_shares_db, k, {}) + 
-                                        {attestation_share}
-                                    ];
-                        
-            if construct_signed_attestation_signature(attestation_shares_db[k]).isPresent()
+            var activate_att_consensus_intances := att_consensus.get_active_instances();
+
+            if 
+                || (activate_att_consensus_intances == {} && !latest_attestation_duty.isPresent())
+                || (activate_att_consensus_intances != {} && minSet(activate_att_consensus_intances) <= attestation_share.data.slot)
+                || (activate_att_consensus_intances == {} && current_attesation_duty.isPresent() && current_attesation_duty.safe_get().slot <= attestation_share.data.slot)                
+                || (activate_att_consensus_intances == {} && !current_attesation_duty.isPresent() && latest_attestation_duty.isPresent() && latest_attestation_duty.safe_get().slot < attestation_share.data.slot)
             {
-                var aggregated_attestation := 
-                        Attestation(
-                            aggregation_bits := attestation_share.aggregation_bits,
-                            data := attestation_share.data,
-                            signature := construct_signed_attestation_signature(attestation_shares_db[k]).safe_get()
-                        );
-                bn.submit_attestation(aggregated_attestation); 
-            }  
+                // TODO: The check above is not consistent with the clean-up operation done in
+                // listen_for_new_imported_blocks. Here, any share for future slot is accepted, whereas
+                // listen_for_new_imported_blocks cleans up the received shares for any already-decided slot. This
+                // inconsistency should be fixed up by either accepting here only shares with slot higher than the
+                // maximum already-decided slot or changing the clean-up code in listen_for_new_imported_blocks to clean
+                // up only slot lower thant the slot of the current/latest duty 
+                var k := (attestation_share.data, attestation_share.aggregation_bits);
+                var attestation_shares_db_at_slot := getOrDefault(rcvd_attestation_shares, attestation_share.data.slot, map[]);
+                rcvd_attestation_shares := 
+                    rcvd_attestation_shares[
+                        attestation_share.data.slot := 
+                            attestation_shares_db_at_slot[
+                                        k := 
+                                            getOrDefault(attestation_shares_db_at_slot, k, {}) + 
+                                            {attestation_share}
+                                        ]
+                            ];
+                            
+                if construct_signed_attestation_signature(rcvd_attestation_shares[attestation_share.data.slot][k]).isPresent()
+                {
+                    var aggregated_attestation := 
+                            Attestation(
+                                aggregation_bits := attestation_share.aggregation_bits,
+                                data := attestation_share.data,
+                                signature := construct_signed_attestation_signature(rcvd_attestation_shares[attestation_share.data.slot][k]).safe_get()
+                            );
+                    bn.submit_attestation(aggregated_attestation); 
+                } 
+            } 
         }
 
         method listen_for_new_imported_blocks(
             block: BeaconBlock
         ) returns (s: Status)
-        modifies this
+        requires ValidRepr()
+        modifies getRepr()
         {
             var valIndex :- bn.get_validator_index(block.body.state_root, dv_pubkey);
             var i := 0;
 
+            var att_consensus_instances_already_decided := future_att_consensus_instances_already_decided;
+
             while i < |block.body.attestations|
-            // for i := 0 to |block.body.attestations|
+                invariant ValidRepr() && fresh(bn.Repr - old(bn.Repr)) && unchanged(rs) && unchanged(network) && unchanged(att_consensus) && unchanged(this) && unchanged(slashing_db)
             {
                 var a := block.body.attestations[i];
-                var committee :- bn.get_epoch_committees(block.body.state_root, a.data.index);
+
+                var committee:- bn.get_epoch_committees(block.body.state_root, a.data.index);
                 
                 if
                 && a in block.body.attestations
-                // && a.data.slot == process.attestation_duty.slot 
-                // && a.data.index == process.attestation_duty.committee_index
                 && valIndex.Some?
                 && valIndex.v in committee
                 && var i:nat :| i < |committee| && committee[i] == valIndex.v;
                 && i < |a.aggregation_bits|
                 && a.aggregation_bits[i]
-                && (current_attesation_duty.isPresent() ==> a.data.slot >= current_attesation_duty.safe_get().slot)
                 {
-                    future_att_consensus_instances_already_decided := future_att_consensus_instances_already_decided + {a.data.slot};
+                    att_consensus_instances_already_decided := att_consensus_instances_already_decided[a.data.slot := a.data];
                 }
 
                 i := i + 1;
             }
 
+            att_consensus.stop_multiple(att_consensus_instances_already_decided.Keys);
+            // TODO: The clean-up below is not consistent with the check done in listen_for_attestation_shares. See
+            // comment in listen_for_attestation_shares for an explanation.         
+            attestation_shares_to_broadcast := attestation_shares_to_broadcast - att_consensus_instances_already_decided.Keys;
+            rcvd_attestation_shares := rcvd_attestation_shares - att_consensus_instances_already_decided.Keys;
 
-            if current_attesation_duty.isPresent() && current_attesation_duty.safe_get().slot in future_att_consensus_instances_already_decided
+            if latest_attestation_duty.isPresent()
             {
-                att_consensus.stop(current_attesation_duty.safe_get().slot);
-                check_for_next_queued_duty();
-            }                                   
+                var old_instances := 
+                        set i | 
+                            && i in att_consensus_instances_already_decided.Keys
+                            && i <= latest_attestation_duty.safe_get().slot
+                        ;
+                future_att_consensus_instances_already_decided := att_consensus_instances_already_decided - old_instances;
+            }
+            else
+            {
+                future_att_consensus_instances_already_decided := att_consensus_instances_already_decided;
+            }            
+
+            if current_attesation_duty.isPresent() && current_attesation_duty.safe_get().slot in att_consensus_instances_already_decided
+            {
+                update_attestation_slashing_db(att_consensus_instances_already_decided[current_attesation_duty.safe_get().slot]);
+                current_attesation_duty := None;
+                { :- check_for_next_queued_duty();}
+            }
+
+            return Success;                              
         }
 
-        method resend_attestation_share(
-        )
-        modifies this
+        method resend_attestation_share()
+        requires ValidRepr()
+        modifies getRepr()
         {
-            if attestation_share_to_broadcast.isPresent()
-            {
-                network.send_att_share(attestation_share_to_broadcast.safe_get(), peers);
-            }
+            network.send_att_shares(attestation_shares_to_broadcast.Values, peers);
+        }     
+
+        static predicate ValidConstructorRepr(
+            att_consensus: Consensus<AttestationData>, 
+            network: Network,
+            bn: BeaconNode,
+            rs: RemoteSigner,
+            slashing_db: SlashingDB            
+        )
+        reads *
+        {
+            && att_consensus.consensus_instances_started.Values 
+            !! bn.Repr !! network.Repr !! att_consensus.Repr 
+            !! rs.Repr !! slashing_db.Repr
+            && bn.Valid()
+            && rs.Valid()
+            && network.Valid()
+            && att_consensus.Valid()    
+            && slashing_db.Valid()                            
+        }   
+
+        function getChildrenRepr(): set<object?>
+        reads *
+        {
+            this.att_consensus.consensus_instances_started.Values 
+            + this.bn.Repr + this.network.Repr + this.att_consensus.Repr + this.rs.Repr
+            + this.slashing_db.Repr
         }        
-    }    
+
+        function getRepr(): set<object?>
+        reads *
+        {
+            getChildrenRepr() + {this}
+        }
+
+        predicate ValidRepr()
+        reads *
+        {
+            && ValidConstructorRepr(this.att_consensus, this.network, this.bn, this.rs, this.slashing_db)
+            && this
+            !in getChildrenRepr()                                
+        }              
+    }  
+
+    class AttestationConsensusValidityCheck extends ConsensusValidityCheck<AttestationData>
+    {
+        const dv_pubkey: BLSPubkey
+        const attestation_duty: AttestationDuty
+
+        constructor(
+            dv_pubkey: BLSPubkey,
+            slashing_db: SlashingDB,
+            attestation_duty: AttestationDuty
+        )
+        requires slashing_db.Valid()
+        ensures this.dv_pubkey == dv_pubkey
+        ensures this.attestation_duty == attestation_duty
+        ensures this.slashing_db == slashing_db
+        ensures Valid()
+        {
+            this.dv_pubkey := dv_pubkey;
+            this.attestation_duty := attestation_duty;
+            this.slashing_db := slashing_db;
+            Repr := {this} + {slashing_db} + slashing_db.Repr;
+        }
+
+        method is_valid(data: AttestationData) returns (valid: bool)
+        requires Valid()
+        modifies Repr
+        ensures Valid()
+        ensures fresh(Repr - old(Repr))
+        {
+            assert Valid();
+            assert slashing_db.Valid();
+            var attestations := slashing_db.get_attestations(dv_pubkey);
+            Repr := Repr + slashing_db.Repr;
+
+            return consensus_is_valid_attestation_data(attestations, data, this.attestation_duty);             
+        }
+    }      
 }
 
 module DVCNode_Externs
@@ -227,82 +395,90 @@ module DVCNode_Externs
     import opened Types
     import opened CommonFunctions
 
-    class Consensus {
-        ghost var consensus_commands_sent: seq<ConsensusCommand>
+    trait 
+    // See https://github.com/dafny-lang/dafny/issues/1588 for why {:termination false} is needed
+    {:termination false} 
+    {:autocontracts} ConsensusValidityCheck<T>
+    {
+        const slashing_db: SlashingDB
 
-        constructor()
-        {
-            consensus_commands_sent := [];
-        }
+        method is_valid(data: T) returns (validity: bool)
+    }    
 
-        method {:extern} start(
-            id: Slot
+    trait {:autocontracts} Consensus<T(!new, ==)>
+    {
+        ghost var consensus_instances_started: map<Slot, ConsensusValidityCheck<T>>
+
+        method start(
+            id: Slot,
+            validityPredicate: ConsensusValidityCheck<T>
+        ) returns (s: Status)
+        ensures s.Success? <==> id !in old(consensus_instances_started.Keys)
+        ensures s.Success? ==> consensus_instances_started == old(consensus_instances_started)[id := validityPredicate]
+        ensures s.Failure? ==> unchanged(`consensus_instances_started)  
+
+        method stop_multiple(
+            ids: set<Slot>
         )
-        ensures consensus_commands_sent == old(consensus_commands_sent) + [ConsensusCommand.Start(id)]
+        ensures consensus_instances_started == old(consensus_instances_started) - ids
 
-        method {:extern} stop(
-            id: Slot
-        )
-        ensures consensus_commands_sent == old(consensus_commands_sent) + [ConsensusCommand.Stop(id)]        
-    }     
+        method get_active_instances() returns (active_instances: set<Slot>)
+        ensures active_instances == consensus_instances_started.Keys 
+        ensures unchanged(`consensus_instances_started) 
+    }    
 
-    class Network  
+    trait {:autocontracts} Network  
     {
         ghost var att_shares_sent: seq<set<MessaageWithRecipient<AttestationShare>>>;
 
-        constructor()
-        {
-            att_shares_sent := [];
-        }
-
-        method {:extern} send_att_share(att_share: AttestationShare, receipients: set<BLSPubkey>)
+        method send_att_share(att_share: AttestationShare, receipients: set<BLSPubkey>)
         ensures att_shares_sent == old(att_shares_sent)  + [addRecepientsToMessage(att_share, receipients)]
+
+        method send_att_shares(att_shares: set<AttestationShare>, receipients: set<BLSPubkey>)
+        ensures     var setWithRecipient := set att_share | att_share in att_shares :: addRecepientsToMessage(att_share, receipients);
+                    att_shares_sent == old(att_shares_sent)  + [setUnion(setWithRecipient)]
+        ensures unchanged(`att_shares_sent)
+
     }
 
-    class BeaconNode
+    trait {:autocontracts} BeaconNode
     {
         ghost var state_roots_of_imported_blocks: set<Root>;
-        ghost const attestations_submitted: seq<Attestation>; 
+        ghost var attestations_submitted: seq<Attestation>; 
 
-        constructor()
-        {
-            attestations_submitted := [];
-            state_roots_of_imported_blocks := {};
-        }
+        method get_fork_version(s: Slot) returns (v: Version)
+        ensures unchanged(`state_roots_of_imported_blocks)
+        ensures unchanged(`attestations_submitted)
 
-        method {:extern} get_fork_version(s: Slot) returns (v: Version)
-
-        method {:extern} submit_attestation(attestation: Attestation)
+        method submit_attestation(attestation: Attestation)
         ensures attestations_submitted == old(attestations_submitted) + [attestation]
+        ensures unchanged(`state_roots_of_imported_blocks)
 
         // https://ethereum.github.io/beacon-APIs/?urls.primaryName=v1#/Beacon/getEpochCommittees
-        method {:extern} get_epoch_committees(
+        method get_epoch_committees(
             state_id: Root,
             index: CommitteeIndex
         ) returns (s: Status, sv: seq<ValidatorIndex>)
+        ensures unchanged(`state_roots_of_imported_blocks)
+        ensures unchanged(`attestations_submitted)        
         ensures state_id in state_roots_of_imported_blocks <==> s.Success?
         ensures uniqueSeq(sv)  
 
         // https://ethereum.github.io/beacon-APIs/#/Beacon/getStateValidator
-        method {:extern} get_validator_index(
+        method get_validator_index(
             state_id: Root,
             validator_id: BLSPubkey
         ) returns (s: Status, vi: Optional<ValidatorIndex>)
+        ensures unchanged(`state_roots_of_imported_blocks)
+        ensures unchanged(`attestations_submitted)        
         ensures state_id in state_roots_of_imported_blocks <==> s.Success?
     }
 
-    class RemoteSigner
+    trait {:autocontracts} RemoteSigner
     {
         const pubkey: BLSPubkey;
 
-        constructor(
-            pubkey: BLSPubkey
-        )
-        {
-            this.pubkey := pubkey;
-        }
-
-        method {:extern} sign_attestation(
+        method sign_attestation(
             attestation_data: AttestationData, 
             fork_version: Version, 
             signing_root: Root           
@@ -310,5 +486,30 @@ module DVCNode_Externs
         requires signing_root == compute_attestation_signing_root(attestation_data, fork_version)
 
     }
+
+    // NOTE: All methods in this trait MUST be implemented thread-safe.
+    trait {:autocontracts} SlashingDB
+    {
+        ghost var attestations: imaptotal<BLSPubkey, set<SlashingDBAttestation>>;
+        ghost var proposals: imaptotal<BLSPubkey, set<SlashingDBBlock>>
+
+        method add_attestation(attestation: SlashingDBAttestation, pubkey: BLSPubkey)
+        ensures attestations == old(attestations)[pubkey := old(attestations)[pubkey] + {attestation}]
+        ensures unchanged(`proposals)
+
+        method get_attestations(pubkey: BLSPubkey) returns (attestations: set<SlashingDBAttestation>)
+        ensures attestations == this.attestations[pubkey]
+        ensures unchanged(`attestations)
+        ensures unchanged(`proposals)
+
+        method add_proposal(block: SlashingDBBlock, pubkey: BLSPubkey)
+        ensures proposals == old(proposals)[pubkey := old(proposals)[pubkey] + {block}]
+        ensures unchanged(`attestations)
+
+        method get_proposals(pubkey: BLSPubkey) returns (proposals: set<SlashingDBBlock>)
+        ensures proposals == this.proposals[pubkey]
+        ensures unchanged(`attestations)
+        ensures unchanged(`proposals)        
+    }    
 }
 
