src/dvspec/dafny/proof/dvc_implementation_spec_proof.dfy
@@ -1,192 +1,1421 @@
 include "../commons.dfy"
 include "../specification/dvc_spec.dfy"
 
-abstract module DVCNode_Implementation_Proofs refines DVCNode_Implementation
+module DVCNode_Implementation_Proofs refines DVCNode_Implementation
 {
     import opened DVCNode_Spec
     import opened DVCNode_Externs = DVCNode_Externs_Proofs
 
+    function toAttestationConsensusValidityCheckState(
+        acvc: ConsensusValidityCheck<AttestationData>
+    ): AttestationConsensusValidityCheckState
+    requires isAttestationConsensusValidityCheck(acvc)
+    reads acvc, acvc.slashing_db
+    {
+        var attestation_duty := (acvc as AttestationConsensusValidityCheck).attestation_duty;
+        var pubkey := (acvc as AttestationConsensusValidityCheck).dv_pubkey;
+        var attestation_slashing_db := acvc.slashing_db.attestations[pubkey];
+        AttestationConsensusValidityCheckState(
+            attestation_duty := attestation_duty,
+            validityPredicate := (ad: AttestationData) => consensus_is_valid_attestation_data(attestation_slashing_db, ad, attestation_duty)
+        )
+    }    
+
+    predicate isAttestationConsensusValidityCheck(
+        cvc: ConsensusValidityCheck<AttestationData>
+    )
+    reads cvc
+    {
+        cvc is AttestationConsensusValidityCheck
+    }
+
+    function toAttestationConsensusValidityCheck(
+        cvc: ConsensusValidityCheck<AttestationData>
+    ): AttestationConsensusValidityCheck
+    requires isAttestationConsensusValidityCheck(cvc)
+    reads cvc
+    {
+        cvc as AttestationConsensusValidityCheck
+    }
+
+    lemma lemmaMapKeysHasOneEntryInItems<K, V>(m: map<K, V>, k: K)  
+    requires k in m.Keys
+    ensures exists i :: i in m.Items && i.0 == k 
+    {
+        assert (k, m[k]) in m.Items;
+    }
+    
+    function get_attestation_consensus_active_instances(
+        m: map<Slot, ConsensusValidityCheck<AttestationData>>
+    ): (r: map<Slot, AttestationConsensusValidityCheckState>)
+    reads m.Values, set v: ConsensusValidityCheck<AttestationData>  | && v in m.Values  :: v.slashing_db
+    ensures r.Keys <= m.Keys
+    ensures forall k | k in r.Keys :: isAttestationConsensusValidityCheck(m[k]) && r[k] == toAttestationConsensusValidityCheckState(m[k])
+    {  
+            map it | 
+                        && it in m.Items 
+                        && isAttestationConsensusValidityCheck(it.1)
+                    :: 
+                    it.0 := toAttestationConsensusValidityCheckState(it.1)           
+    }
+
+    function toConsensusEngineState(ce: Consensus<AttestationData>): (r: ConsensusEngineState)
+    reads ce, ce.consensus_instances_started.Values, set v: ConsensusValidityCheck<AttestationData>  | && v in ce.consensus_instances_started.Values  :: v.slashing_db
+    {
+        ConsensusEngineState(
+            attestation_consensus_active_instances := get_attestation_consensus_active_instances(ce.consensus_instances_started)   
+        )
+    }
+
+    twostate predicate lemmaConsensusInstancesHaveBeenRemovedPrecond(
+        ce: Consensus<AttestationData>,
+        removed_keys: set<Slot>
+    )
+    reads ce, ce.consensus_instances_started.Values, set v: ConsensusValidityCheck<AttestationData>  | && v in ce.consensus_instances_started.Values  :: v.slashing_db
+    {
+        ce.consensus_instances_started == old(ce.consensus_instances_started) - removed_keys 
+        && forall v | v in ce.consensus_instances_started.Values :: 
+            && old(allocated(v))
+            && unchanged(v.slashing_db)
+            && unchanged(v)   
+    }    
+
+    twostate lemma lemmaConsensusInstancesHaveBeenRemoved(
+        ce: Consensus<AttestationData>,
+        removed_keys: set<Slot>
+    )
+    requires lemmaConsensusInstancesHaveBeenRemovedPrecond(ce, removed_keys)
+    ensures toConsensusEngineState(ce) == old(toConsensusEngineState(ce)).(
+        attestation_consensus_active_instances := old(toConsensusEngineState(ce)).attestation_consensus_active_instances - removed_keys
+    )
+    {      
+    }    
+
+    twostate predicate lemmaConsensusInstancesAreTheSamePrecond(
+        ce: Consensus<AttestationData>
+    )
+    reads ce, ce.consensus_instances_started.Values, set v: ConsensusValidityCheck<AttestationData>  | && v in ce.consensus_instances_started.Values  :: v.slashing_db
+    {
+        && unchanged(ce)
+        && forall v | v in ce.consensus_instances_started.Values :: 
+            && old(allocated(v))
+            && isAttestationConsensusValidityCheck(v) 
+            && unchanged(v.slashing_db) 
+            && unchanged(v)   
+    }
+
+    twostate lemma lemmaConsensusInstancesAreTheSame(
+        ce: Consensus<AttestationData>
+    )
+    requires lemmaConsensusInstancesAreTheSamePrecond(ce)
+    ensures old(toConsensusEngineState(ce)) == toConsensusEngineState(ce)
+    {
+
+        forall e | e in old(toConsensusEngineState(ce)).attestation_consensus_active_instances.Keys
+        ensures e in toConsensusEngineState(ce).attestation_consensus_active_instances.Keys;
+        {
+            lemmaMapKeysHasOneEntryInItems(old(toConsensusEngineState(ce)).attestation_consensus_active_instances, e);
+        } 
+
+        assert old(toConsensusEngineState(ce)).attestation_consensus_active_instances.Keys == toConsensusEngineState(ce).attestation_consensus_active_instances.Keys;        
+    }
+
     export PublicInterface...
         reveals *
 
-    function toDVCNodeState(n: DVCNode): DVCNodeState
-    reads n, n.bn, n.rs
-    {
-        DVCNodeState(
-            current_attesation_duty := n.current_attesation_duty,
-            attestation_duties_queue := n.attestation_duties_queue,
-            attestation_slashing_db := n.attestation_slashing_db,
-            attestation_shares_db := n.attestation_shares_db,
-            attestation_share_to_broadcast := n.attestation_share_to_broadcast,
-            peers := n.peers,
-            construct_signed_attestation_signature := n.construct_signed_attestation_signature,
-            dv_pubkey := n.dv_pubkey,
-            future_att_consensus_instances_already_decided := n.future_att_consensus_instances_already_decided,
-            bn := toBNState(n.bn),
-            rs := toRSState(n.rs)
-        )
-    }
-
-    function seqToSet<T>(s: seq<T>): (r: set<T>)
-    {
-        set e | e in s
-    }
-
     function seqMinusToSet<T>(s1: seq<T>, s2: seq<T>): set<T>
-    // requires s2 <= s1 
-    // ensures seqMinus(s1, s2) + s2 == s1
     {
-        set i | |s2| <= i < |s1| :: s1[i]
-    }
-
-    function seqMinusToOptional<T>(s1: seq<T>, s2: seq<T>): Optional<T>
-    requires s2 <= s1 
-    requires |s1| <= |s2| + 1
-    {
-        if s1 == s2 then
-            None 
+        if |s2| <= |s1| then
+            var seqDiff := s1[|s2|..];
+            assert s2 <= s1 ==> s2 + seqDiff == s1;
+            seqToSet(seqDiff)
         else
-            Some(s1[|s2|])
+            {}
     }
-
-
-
-
-
-
-    twostate predicate onlyOneMaxConsensusCommandAndSubmittedAttestation(n: DVCNode)
-    reads n, n.att_consensus, n.bn
-    {
-        && |n.att_consensus.consensus_commands_sent| <= |old(n.att_consensus.consensus_commands_sent)| + 1
-        && |n.bn.attestations_submitted| <= |old(n.bn.attestations_submitted)| + 1
-    }
-
-    twostate function getOutputs(n: DVCNode): (o: Outputs)
-    reads n, n.network, n.att_consensus, n.bn
-    {
-        Outputs(
-            att_shares_sent :=  setUnion(seqMinusToSet(n.network.att_shares_sent, old(n.network.att_shares_sent))),
-            att_consensus_commands_sent := seqMinusToSet(n.att_consensus.consensus_commands_sent, old(n.att_consensus.consensus_commands_sent)),
-            attestations_submitted := seqMinusToSet(n.bn.attestations_submitted, old(n.bn.attestations_submitted))
-        )
-    }
-
-    
-
-    twostate function toDVCNodeStateAndOuputs(n: DVCNode): DVCNodeStateAndOuputs
-    reads n, n.network, n.att_consensus, n.bn, n.rs
-    {
-        DVCNodeStateAndOuputs(
-            state := toDVCNodeState(n),
-            outputs := getOutputs(n)
-        )
-    }
-
- 
-
-
-
 
     class DVCNode...
     {
-
-        method update_attestation_slashing_db...
-        ensures f_update_attestation_slashing_db(old(toDVCNodeState(this)).attestation_slashing_db, attestation_data, attestation_duty_pubkey) == this.attestation_slashing_db;  
-
-        method serve_attestation_duty...
-        ensures f_serve_attestation_duty(old(toDVCNodeState(this)), attestation_duty) == toDVCNodeStateAndOuputs(this);
+        function toDVCNodeState(): DVCNodeState
+        reads this, bn, rs, att_consensus, slashing_db, att_consensus.consensus_instances_started.Values, set v: ConsensusValidityCheck<AttestationData>  | && v in att_consensus.consensus_instances_started.Values  :: v.slashing_db
         {
-            ...;
-            assert f_serve_attestation_duty(old(toDVCNodeState(this)), attestation_duty) == toDVCNodeStateAndOuputs(this);
+            DVCNodeState(
+                current_attesation_duty := current_attesation_duty,
+                latest_attestation_duty := latest_attestation_duty,
+                attestation_duties_queue := attestation_duties_queue,
+                attestation_slashing_db := slashing_db.attestations[dv_pubkey],
+                rcvd_attestation_shares := rcvd_attestation_shares,
+                attestation_shares_to_broadcast := attestation_shares_to_broadcast,
+                attestation_consensus_engine_state := toConsensusEngineState(att_consensus),
+                peers := peers,
+                construct_signed_attestation_signature := construct_signed_attestation_signature,
+                dv_pubkey := dv_pubkey,
+                future_att_consensus_instances_already_decided := future_att_consensus_instances_already_decided,
+                bn := toBNState(bn),
+                rs := toRSState(rs)
+            )
+        }  
+
+        twostate function getOutputs(): (o: Outputs)
+        reads this, network, bn
+        {
+            Outputs(
+                att_shares_sent :=  setUnion(seqMinusToSet(network.att_shares_sent, old(network.att_shares_sent))),
+                attestations_submitted := seqMinusToSet(bn.attestations_submitted, old(bn.attestations_submitted))
+            )
+        }              
+
+        twostate function toDVCNodeStateAndOuputs(): DVCNodeStateAndOuputs
+        reads this, network, att_consensus, bn, rs, slashing_db, att_consensus.consensus_instances_started.Values, set v: ConsensusValidityCheck<AttestationData>  | && v in att_consensus.consensus_instances_started.Values :: v.slashing_db
+        {
+            DVCNodeStateAndOuputs(
+                state := toDVCNodeState(),
+                outputs := getOutputs()
+            )
+        }        
+
+        predicate isValidReprExtended()
+        reads *
+        {
+            && (forall vp | vp in att_consensus.consensus_instances_started.Values :: 
+                        && isAttestationConsensusValidityCheck(vp)
+                        && vp.slashing_db == this.slashing_db
+                        && toAttestationConsensusValidityCheck(vp).dv_pubkey == this.dv_pubkey
+            )
+            && ValidRepr()
         }
 
+        constructor...
+        ensures 
+                && isValidReprExtended()
+                && Init(toDVCNodeState(), dv_pubkey, peers, construct_signed_attestation_signature, initial_slashing_db.attestations[dv_pubkey], rs.pubkey)
+        {
+            ...;
+        }
+
+        method process_event...
+        ensures (old(isValidReprExtended()) && f_process_event.requires(old(toDVCNodeState()), event)) ==>    
+                && isValidReprExtended()
+                && f_process_event(old(toDVCNodeState()), event) == toDVCNodeStateAndOuputs()
+                && s.Success?        
+        {
+            ...; 
+
+            {
+                if event.ServeAttstationDuty?
+                {    
+                    assert (old(isValidReprExtended()) && f_process_event.requires(old(toDVCNodeState()), event)) ==> 
+                        && f_process_event(old(toDVCNodeState()), event) == toDVCNodeStateAndOuputs()
+                        && isValidReprExtended();
+                }
+                else if event.AttConsensusDecided?
+                {
+                    assert (old(isValidReprExtended()) && f_process_event.requires(old(toDVCNodeState()), event)) ==> 
+                        && f_process_event(old(toDVCNodeState()), event) == toDVCNodeStateAndOuputs()
+                        && isValidReprExtended();       
+                }         
+                else if event.ReceviedAttesttionShare?
+                {    
+                    assert (old(isValidReprExtended()) && f_process_event.requires(old(toDVCNodeState()), event)) ==> 
+                        && f_process_event(old(toDVCNodeState()), event) == toDVCNodeStateAndOuputs()
+                        && isValidReprExtended();  
+                }              
+                else if event.ImportedNewBlock? 
+                {    assert (old(isValidReprExtended()) && f_process_event.requires(old(toDVCNodeState()), event)) ==> 
+                        && f_process_event(old(toDVCNodeState()), event) == toDVCNodeStateAndOuputs()
+                        && isValidReprExtended();  
+                }              
+                else if event.ResendAttestationShares?
+                {    
+                    assert (old(isValidReprExtended()) && f_process_event.requires(old(toDVCNodeState()), event)) ==> 
+                        && f_process_event(old(toDVCNodeState()), event) == toDVCNodeStateAndOuputs()
+                        && isValidReprExtended(); 
+                }               
+                else
+                {    
+                    assert (old(isValidReprExtended()) && f_process_event.requires(old(toDVCNodeState()), event)) ==> 
+                        && f_process_event(old(toDVCNodeState()), event) == toDVCNodeStateAndOuputs()
+                        && isValidReprExtended(); 
+                }                   
+                ...;
+            }   
+        }
+
+        method serve_attestation_duty...
+        ensures (old(isValidReprExtended()) && f_serve_attestation_duty.requires(old(toDVCNodeState()), attestation_duty)) ==> 
+                && f_serve_attestation_duty(old(toDVCNodeState()), attestation_duty) == toDVCNodeStateAndOuputs()
+                && isValidReprExtended()
+                && s.Success?
+                && unchanged(network)
+                && unchanged(bn)
+                && unchanged(rs)                
+        {
+            ...;
+            {
+                var o := toDVCNodeState();
+                ...;
+                assert o == old(toDVCNodeState()).(
+                            attestation_duties_queue := old(toDVCNodeState()).attestation_duties_queue + [attestation_duty]
+                        );
+                assert (old(isValidReprExtended()) && f_serve_attestation_duty.requires(old(toDVCNodeState()), attestation_duty)) ==> f_serve_attestation_duty(old(toDVCNodeState()), attestation_duty) == toDVCNodeStateAndOuputs();
+            }
+
+        }
+
+        function  f_check_for_next_queued_duty_helper(process: DVCNodeState): DVCNodeState
+        requires forall ad | ad in process.attestation_duties_queue :: ad.slot !in process.attestation_consensus_engine_state.attestation_consensus_active_instances.Keys
+        requires process.attestation_duties_queue != []
+        requires process.attestation_duties_queue[0].slot in process.future_att_consensus_instances_already_decided.Keys 
+        decreases process.attestation_duties_queue
+        {
+            var queue_head := process.attestation_duties_queue[0];
+            var new_attestation_slashing_db := f_update_attestation_slashing_db(process.attestation_slashing_db, process.future_att_consensus_instances_already_decided[queue_head.slot]);
+            process.(
+                attestation_duties_queue := process.attestation_duties_queue[1..],
+                future_att_consensus_instances_already_decided := process.future_att_consensus_instances_already_decided - {queue_head.slot},
+                attestation_slashing_db := new_attestation_slashing_db,
+                attestation_consensus_engine_state := updateConsensusInstanceValidityCheck(
+                    process.attestation_consensus_engine_state,
+                    new_attestation_slashing_db
+                )                        
+            )
+        }          
+
         method check_for_next_queued_duty...
-        ensures f_check_for_next_queued_duty(old(toDVCNodeState(this))) == toDVCNodeStateAndOuputs(this);
+        ensures (old(isValidReprExtended()) && f_check_for_next_queued_duty.requires(old(toDVCNodeState())))==> 
+                && f_check_for_next_queued_duty(old(toDVCNodeState())) == toDVCNodeStateAndOuputs()
+                && isValidReprExtended()
+                && s.Success?
+                && unchanged(network)
+                && unchanged(bn)
+                && unchanged(rs)   
+                && unchanged(`rcvd_attestation_shares)
+                && unchanged(`attestation_shares_to_broadcast)
+                && unchanged(`construct_signed_attestation_signature)
+                && unchanged(`peers)
+                && unchanged(`dv_pubkey)
+                && fresh(att_consensus.Repr - old(att_consensus.Repr))                     
+
         {
             if...
             {
                 if...
                 {
                     ...;
-                    assert f_check_for_next_queued_duty(old(toDVCNodeState(this))) == toDVCNodeStateAndOuputs(this);
+                    {                      
+                        if (old(isValidReprExtended()) && f_check_for_next_queued_duty.requires(old(toDVCNodeState()))) 
+                        {
+                            var rs := f_check_for_next_queued_duty_helper(old(toDVCNodeState()));                              
+
+                            forall e | e in old(toDVCNodeState()).attestation_consensus_engine_state.attestation_consensus_active_instances.Keys
+                            ensures e in rs.attestation_consensus_engine_state.attestation_consensus_active_instances.Keys
+                            {
+                                lemmaMapKeysHasOneEntryInItems(old(toDVCNodeState()).attestation_consensus_engine_state.attestation_consensus_active_instances, e);
+                            }   
+
+                            lemmaAttestationHasBeenAddedToSlashingDb(old(future_att_consensus_instances_already_decided)[queue_head.slot], rs);                       
+                                                    
+                            assert f_check_for_next_queued_duty_helper(old(toDVCNodeState())) == toDVCNodeState(); 
+
+                        }
+                       
+                        ...;
+
+                        assert (old(isValidReprExtended()) && f_check_for_next_queued_duty.requires(old(toDVCNodeState()))) ==> f_check_for_next_queued_duty(old(toDVCNodeState())) == toDVCNodeStateAndOuputs();       
+                    }
+
+                }
+                else if...
+                {
+                    ...;
+                    assert (old(isValidReprExtended()) && f_check_for_next_queued_duty.requires(old(toDVCNodeState()))) ==> f_check_for_next_queued_duty(old(toDVCNodeState())) == toDVCNodeStateAndOuputs();
                 }
                 else
                 {
-                    ...;
-                    assert f_check_for_next_queued_duty(old(toDVCNodeState(this))) == toDVCNodeStateAndOuputs(this);
+                    assert (old(isValidReprExtended()) && f_check_for_next_queued_duty.requires(old(toDVCNodeState()))) ==> f_check_for_next_queued_duty(old(toDVCNodeState())) == toDVCNodeStateAndOuputs();
                 }
             }
             else
             {
-                assert f_check_for_next_queued_duty(old(toDVCNodeState(this))) == toDVCNodeStateAndOuputs(this);
+                assert (old(isValidReprExtended()) && f_check_for_next_queued_duty.requires(old(toDVCNodeState()))) ==> f_check_for_next_queued_duty(old(toDVCNodeState())) == toDVCNodeStateAndOuputs();
             }
+        }     
+
+        method start_next_duty...
+        ensures 
+                old(isValidReprExtended()) ==>
+                (
+                    && isValidReprExtended()
+                    && (f_start_next_duty.requires(old(toDVCNodeState()), attestation_duty) ==> 
+                        && (f_start_next_duty(old(toDVCNodeState()), attestation_duty) == toDVCNodeStateAndOuputs())
+                        && s.Success?
+                        && unchanged(network)
+                        && unchanged(bn)
+                        && unchanged(rs)
+                        && current_attesation_duty == Some(attestation_duty)
+                        && latest_attestation_duty == Some(attestation_duty)
+                        && unchanged(`attestation_duties_queue)
+                        && unchanged(slashing_db)
+                        && unchanged(`rcvd_attestation_shares)
+                        && unchanged(`attestation_shares_to_broadcast)
+                        && unchanged(`construct_signed_attestation_signature)
+                        && unchanged(`peers)
+                        && unchanged(`dv_pubkey)
+                        && unchanged(`future_att_consensus_instances_already_decided)
+                        && att_consensus.consensus_instances_started.Keys == old(att_consensus.consensus_instances_started.Keys) + {attestation_duty.slot}
+                        && fresh(att_consensus.Repr - old(att_consensus.Repr))
+                    )
+                )
+        {
+            if old(isValidReprExtended())
+            {
+                forall e | e in old(att_consensus.consensus_instances_started.Keys)
+                ensures e in old(get_attestation_consensus_active_instances(att_consensus.consensus_instances_started)).Keys; // TOOD: Possible violation of postcondition
+                {
+                    lemmaMapKeysHasOneEntryInItems(old(att_consensus.consensus_instances_started), e);
+                }     
+            }                 
+            ...;
+            {
+                ...;
+            }
+            if old(isValidReprExtended())
+            {
+                lemmaMapKeysHasOneEntryInItems(att_consensus.consensus_instances_started, attestation_duty.slot);
+                                                                                     
+                assert f_start_next_duty(old(toDVCNodeState()), attestation_duty) == toDVCNodeStateAndOuputs();
+            }
+        }
+
+        method update_attestation_slashing_db...
+        ensures f_update_attestation_slashing_db(old(toDVCNodeState()).attestation_slashing_db, attestation_data) == this.slashing_db.attestations[this.dv_pubkey] == toDVCNodeState().attestation_slashing_db
+        ensures  var slashing_db_attestation := SlashingDBAttestation(
+                                                source_epoch := attestation_data.source.epoch,
+                                                target_epoch := attestation_data.target.epoch,
+                                                signing_root := Some(hash_tree_root(attestation_data)));
+            slashing_db.attestations == old(slashing_db.attestations)[dv_pubkey := old(slashing_db.attestations)[dv_pubkey] + {slashing_db_attestation}]
+        ensures && unchanged(slashing_db`proposals)
+                && unchanged(this)
+                && unchanged(network)
+                && unchanged(rs)
+                && unchanged(bn)
+                && unchanged(att_consensus)
+                && unchanged(att_consensus.consensus_instances_started.Values)
+        {
+            ...;
+        }
+
+        function f_att_consensus_decided_helper(
+            process: DVCNodeState,
+            id: Slot,
+            decided_attestation_data: AttestationData
+        ): DVCNodeStateAndOuputs
+        requires process.current_attesation_duty.isPresent()
+        requires forall ad | ad in process.attestation_duties_queue :: ad.slot !in process.attestation_consensus_engine_state.attestation_consensus_active_instances.Keys    
+        {
+            var local_current_attestation_duty := process.current_attesation_duty.safe_get();
+            var attestation_slashing_db := f_update_attestation_slashing_db(process.attestation_slashing_db, decided_attestation_data);
+
+            var fork_version := bn_get_fork_version(compute_start_slot_at_epoch(decided_attestation_data.target.epoch));
+            var attestation_signing_root := compute_attestation_signing_root(decided_attestation_data, fork_version);
+            var attestation_signature_share := rs_sign_attestation(decided_attestation_data, fork_version, attestation_signing_root, process.rs);
+            var attestation_with_signature_share := AttestationShare(
+                    aggregation_bits := get_aggregation_bits(local_current_attestation_duty.validator_index),
+                    data := decided_attestation_data, 
+                    signature := attestation_signature_share
+                ); 
+
+            var newProcess := 
+                process.(
+                    current_attesation_duty := None,
+                    attestation_shares_to_broadcast := process.attestation_shares_to_broadcast[local_current_attestation_duty.slot := attestation_with_signature_share],
+                    attestation_slashing_db := attestation_slashing_db,
+                    attestation_consensus_engine_state := updateConsensusInstanceValidityCheck(
+                        process.attestation_consensus_engine_state,
+                        attestation_slashing_db
+                    )
+                )
+                ;
+
+            DVCNodeStateAndOuputs(
+                newProcess,
+                outputs := getEmptyOuputs().(
+                    att_shares_sent := multicast(attestation_with_signature_share, process.peers)
+                )                  
+            )                
+        }  
+
+        twostate lemma lemmaAttestationHasBeenAddedToSlashingDbForall(
+            attestation_data: AttestationData
+        )
+        requires old(isValidReprExtended())
+        requires isValidReprExtended()
+        requires unchanged(att_consensus)
+        requires var slashing_db_attestation := SlashingDBAttestation(
+                                                source_epoch := attestation_data.source.epoch,
+                                                target_epoch := attestation_data.target.epoch,
+                                                signing_root := Some(hash_tree_root(attestation_data)));        
+                && slashing_db.attestations == old(slashing_db.attestations)[dv_pubkey := old(slashing_db.attestations)[dv_pubkey] + {slashing_db_attestation}]
+        ensures
+                forall p: DVCNodeState |
+                        && p.dv_pubkey == dv_pubkey  
+                        && var new_attestation_slashing_db := f_update_attestation_slashing_db(old(toDVCNodeState()).attestation_slashing_db, attestation_data);
+                        && p.attestation_slashing_db == f_update_attestation_slashing_db(old(toDVCNodeState()).attestation_slashing_db, attestation_data)
+                        && p.attestation_consensus_engine_state == updateConsensusInstanceValidityCheck(
+                            old(toDVCNodeState()).attestation_consensus_engine_state,
+                            new_attestation_slashing_db
+                        )
+                    ::  
+                        p.attestation_consensus_engine_state ==  toDVCNodeState().attestation_consensus_engine_state
+        {
+            forall p: DVCNodeState |
+                && p.dv_pubkey == dv_pubkey  
+                && var new_attestation_slashing_db := f_update_attestation_slashing_db(old(toDVCNodeState()).attestation_slashing_db, attestation_data);
+                && p.attestation_slashing_db == f_update_attestation_slashing_db(old(toDVCNodeState()).attestation_slashing_db, attestation_data)
+                && p.attestation_consensus_engine_state == updateConsensusInstanceValidityCheck(
+                    old(toDVCNodeState()).attestation_consensus_engine_state,
+                    new_attestation_slashing_db
+                )
+            ensures  p.attestation_consensus_engine_state ==  toDVCNodeState().attestation_consensus_engine_state
+            {
+                forall e | e in old(toDVCNodeState()).attestation_consensus_engine_state.attestation_consensus_active_instances.Keys
+                ensures e in p.attestation_consensus_engine_state.attestation_consensus_active_instances.Keys
+                {
+                    lemmaMapKeysHasOneEntryInItems(old(toDVCNodeState()).attestation_consensus_engine_state.attestation_consensus_active_instances, e);
+                } 
+            }                  
+        }
+
+        twostate lemma lemmaAttestationHasBeenAddedToSlashingDb(
+            attestation_data: AttestationData,
+            p: DVCNodeState
+        )
+        requires old(isValidReprExtended())
+        requires isValidReprExtended()
+        requires unchanged(att_consensus)
+        requires var slashing_db_attestation := SlashingDBAttestation(
+                                                source_epoch := attestation_data.source.epoch,
+                                                target_epoch := attestation_data.target.epoch,
+                                                signing_root := Some(hash_tree_root(attestation_data)));        
+                && slashing_db.attestations == old(slashing_db.attestations)[dv_pubkey := old(slashing_db.attestations)[dv_pubkey] + {slashing_db_attestation}]
+        requires
+
+                        && p.dv_pubkey == dv_pubkey  
+                        && var new_attestation_slashing_db := f_update_attestation_slashing_db(old(toDVCNodeState()).attestation_slashing_db, attestation_data);
+                        && p.attestation_slashing_db == f_update_attestation_slashing_db(old(toDVCNodeState()).attestation_slashing_db, attestation_data)
+                        && p.attestation_consensus_engine_state == updateConsensusInstanceValidityCheck(
+                            old(toDVCNodeState()).attestation_consensus_engine_state,
+                            new_attestation_slashing_db
+                        )
+        ensures
+                        p.attestation_consensus_engine_state ==  toDVCNodeState().attestation_consensus_engine_state
+        {
+            forall e | e in old(toDVCNodeState()).attestation_consensus_engine_state.attestation_consensus_active_instances.Keys
+            ensures e in p.attestation_consensus_engine_state.attestation_consensus_active_instances.Keys
+            {
+                lemmaMapKeysHasOneEntryInItems(old(toDVCNodeState()).attestation_consensus_engine_state.attestation_consensus_active_instances, e);
+            }           
+        }                        
+
+        method att_consensus_decided...
+        ensures (old(isValidReprExtended()) && f_att_consensus_decided.requires(old(toDVCNodeState()), id, decided_attestation_data)) ==> 
+                && f_att_consensus_decided(old(toDVCNodeState()), id, decided_attestation_data) == toDVCNodeStateAndOuputs()
+                && isValidReprExtended()
+                && r.Success?
+        {
+            ...;
+            {
+                if old(isValidReprExtended()) && f_att_consensus_decided.requires(old(toDVCNodeState()), id, decided_attestation_data)
+                {
+                    var r := f_att_consensus_decided_helper(old(toDVCNodeState()), id, decided_attestation_data);
+                    var s := old(current_attesation_duty).safe_get().slot;
+                    var rs := r.state;
+
+                    lemmaAttestationHasBeenAddedToSlashingDb(decided_attestation_data, rs); 
+
+                    assert f_att_consensus_decided_helper(old(toDVCNodeState()), id, decided_attestation_data).state == toDVCNodeStateAndOuputs().state; 
+                }                
+                ...;
+            }
+            ...;
+        }
+
+        function method get_aggregation_bits...
+        ensures 
+                var s := get_aggregation_bits(index);
+                && |s| == index
+                && forall i | 0 <= i < |s| :: if i == index - 1 then s[i] else !s[i]         
+
+        // Helper functions/lemmas used when proving the postcondition of method listen_for_attestation_shares below
+        predicate f_listen_for_attestation_shares_helper_2(
+            process: DVCNodeState,
+            attestation_share: AttestationShare
+        )
+        {
+            var activate_att_consensus_intances := process.attestation_consensus_engine_state.attestation_consensus_active_instances.Keys;
+
+                || (activate_att_consensus_intances == {} && !process.latest_attestation_duty.isPresent())
+                || (activate_att_consensus_intances != {} && minSet(activate_att_consensus_intances) <= attestation_share.data.slot)
+                || (activate_att_consensus_intances == {} && process.current_attesation_duty.isPresent() && process.current_attesation_duty.safe_get().slot <= attestation_share.data.slot)                
+                || (activate_att_consensus_intances == {} && !process.current_attesation_duty.isPresent() && process.latest_attestation_duty.isPresent() && process.latest_attestation_duty.safe_get().slot < attestation_share.data.slot)     
+        } 
+
+        function f_listen_for_attestation_shares_helper(
+            process: DVCNodeState,
+            attestation_share: AttestationShare
+        ): DVCNodeState
+        {
+            var activate_att_consensus_intances := process.attestation_consensus_engine_state.attestation_consensus_active_instances.Keys;
+
+            var k := (attestation_share.data, attestation_share.aggregation_bits);
+            var attestation_shares_db_at_slot := getOrDefault(process.rcvd_attestation_shares, attestation_share.data.slot, map[]);
+            
+            var new_attestation_shares_db := 
+                    process.rcvd_attestation_shares[
+                        attestation_share.data.slot := 
+                            attestation_shares_db_at_slot[
+                                        k := 
+                                            getOrDefault(attestation_shares_db_at_slot, k, {}) + 
+                                            {attestation_share}
+                                        ]
+                            ];
+
+            process.(
+                rcvd_attestation_shares := new_attestation_shares_db
+            )
+        }        
+
+        method listen_for_attestation_shares...
+        ensures old(isValidReprExtended()) ==> 
+                        && isValidReprExtended()
+                        && f_listen_for_attestation_shares(old(toDVCNodeState()), attestation_share) == toDVCNodeStateAndOuputs();
+        {
+            ...;
+            if...
+            {
+                if  old(isValidReprExtended())
+                {
+                    forall e | e in old(toDVCNodeState()).attestation_consensus_engine_state.attestation_consensus_active_instances.Keys
+                    ensures e in att_consensus.consensus_instances_started.Keys
+                    {
+                        lemmaMapKeysHasOneEntryInItems(old(toDVCNodeState()).attestation_consensus_engine_state.attestation_consensus_active_instances, e);
+                    }                 
+                    forall e | e in att_consensus.consensus_instances_started.Keys
+                    ensures e in old(toDVCNodeState()).attestation_consensus_engine_state.attestation_consensus_active_instances.Keys;
+                    {
+                        lemmaMapKeysHasOneEntryInItems(att_consensus.consensus_instances_started, e);
+                    }                  
+                    assert att_consensus.consensus_instances_started.Keys <= old(toDVCNodeState()).attestation_consensus_engine_state.attestation_consensus_active_instances.Keys;
+                    assert old(isValidReprExtended()) ==>  f_listen_for_attestation_shares_helper_2(old(toDVCNodeState()), attestation_share);
+                }
+                ...;
+                if...
+                {
+                assert old(isValidReprExtended()) ==> 
+                        && isValidReprExtended()
+                        && f_listen_for_attestation_shares_helper(old(toDVCNodeState()), attestation_share) == toDVCNodeState();                      
+                    ...;
+                }
+                assert old(isValidReprExtended()) ==> 
+                        && isValidReprExtended()
+                        && f_listen_for_attestation_shares(old(toDVCNodeState()), attestation_share).state == f_listen_for_attestation_shares_helper(old(toDVCNodeState()), attestation_share);
+                assert old(isValidReprExtended()) ==> 
+                        && isValidReprExtended()
+                        && f_listen_for_attestation_shares(old(toDVCNodeState()), attestation_share).state == toDVCNodeState();                          
+            }
+            else
+            {
+                assert old(isValidReprExtended()) ==> 
+                            && isValidReprExtended()
+                            && f_listen_for_attestation_shares(old(toDVCNodeState()), attestation_share) == toDVCNodeStateAndOuputs();
+            }
+        }
+
+        // Helper function/lemmas used when proving the postcondition of method listen_for_new_imported_blocks below
+        function f_listen_for_new_imported_blocks_part_1_for_loop_inv(
+            process: DVCNodeState,
+            block: BeaconBlock,
+            i: nat
+        ) : (new_att: map<Slot, AttestationData>)
+        requires i <= |block.body.attestations|
+        requires f_listen_for_new_imported_blocks.requires(process, block)
+        {            
+            map a |
+                    && a in block.body.attestations[..i]
+                    && isMyAttestation(a, process, block, bn_get_validator_index(process.bn, block.body.state_root, process.dv_pubkey))
+                ::
+                    a.data.slot := a.data
+        }  
+
+        predicate p_listen_for_new_imported_blocks_part_2_for_loop_inv(
+            process: DVCNodeState,
+            block: BeaconBlock,
+            i: nat,
+            a2: map<Slot, AttestationData>
+        ) 
+        requires i <= |block.body.attestations|
+        requires f_listen_for_new_imported_blocks.requires(process, block)
+        {
+            a2 == process.future_att_consensus_instances_already_decided + f_listen_for_new_imported_blocks_part_1_for_loop_inv(process, block, i)
+        }        
+
+        lemma lemma_f_listen_for_new_imported_blocks_part_1_to_2_for_loop_inv(
+            process: DVCNodeState,
+            block: BeaconBlock,
+            i: nat,
+            a1: map<Slot, AttestationData>,
+            a2: map<Slot, AttestationData>
+        ) 
+        requires i < |block.body.attestations|
+        requires f_listen_for_new_imported_blocks.requires(process, block)        
+        requires var valIndex := bn_get_validator_index(process.bn, block.body.state_root, process.dv_pubkey);
+                && a1 == process.future_att_consensus_instances_already_decided + f_listen_for_new_imported_blocks_part_1_for_loop_inv(process, block, i)
+                && var a := block.body.attestations[i]; a2 == if isMyAttestation(a,process, block, valIndex) then 
+                            a1[a.data.slot := a.data]
+                        else 
+                            a1
+        ensures p_listen_for_new_imported_blocks_part_2_for_loop_inv(process, block, i + 1, a2)
+        {
+            // Yes!!! The following is needed to allow Dafny prove the lemma!!!
+            var a := block.body.attestations[i];
+            if isMyAttestation(a,process, block, bn_get_validator_index(process.bn, block.body.state_root, process.dv_pubkey)) 
+            {
+                
+            }
+        }
+
+        predicate p_listen_for_new_imported_blocks_part_2(
+            process: DVCNodeState,
+            block: BeaconBlock,
+            a1: map<Slot, AttestationData>
+        ) 
+        requires f_listen_for_new_imported_blocks_part_1.requires(process, block)
+        {
+            a1 == process.future_att_consensus_instances_already_decided + f_listen_for_new_imported_blocks_part_1(process, block)
+        }
+
+
+        lemma lemma_p_listen_for_new_imported_blocks_part_2_for_loop_inv_to_part_2(
+            process: DVCNodeState,
+            block: BeaconBlock,
+            a1: map<Slot, AttestationData>
+        ) 
+        requires f_listen_for_new_imported_blocks.requires(process, block)        
+        requires    var valIndex := bn_get_validator_index(process.bn, block.body.state_root, process.dv_pubkey);
+                    p_listen_for_new_imported_blocks_part_2_for_loop_inv(process, block,|block.body.attestations|, a1)
+        ensures a1 == process.future_att_consensus_instances_already_decided + f_listen_for_new_imported_blocks_part_1(process, block);
+        ensures p_listen_for_new_imported_blocks_part_2(process, block, a1)
+        ensures f_listen_for_new_imported_blocks_part_2(process, block).attestation_consensus_engine_state.attestation_consensus_active_instances == process.attestation_consensus_engine_state.attestation_consensus_active_instances - a1.Keys
+        {
 
         }        
 
-        method start_next_duty...
-        ensures f_start_next_duty(old(toDVCNodeState(this)), attestation_duty) == toDVCNodeStateAndOuputs(this);
+        function f_listen_for_new_imported_blocks_part_1(
+            process: DVCNodeState,
+            block: BeaconBlock
+        ): map<Slot, AttestationData>
+       requires f_listen_for_new_imported_blocks.requires(process, block)       
         {
-            ...;
-            assert f_start_next_duty(old(toDVCNodeState(this)), attestation_duty) == toDVCNodeStateAndOuputs(this);
+            var valIndex := bn_get_validator_index(process.bn, block.body.state_root, process.dv_pubkey);
+                
+            map a |
+                    && a in block.body.attestations
+                    && isMyAttestation(a, process, block, valIndex)
+                ::
+                    a.data.slot := a.data
+
+        }         
+
+        function f_listen_for_new_imported_blocks_part_2(
+            process: DVCNodeState,
+            block: BeaconBlock
+        ): DVCNodeState
+        requires f_listen_for_new_imported_blocks.requires(process, block)        
+        {
+            var valIndex := bn_get_validator_index(process.bn, block.body.state_root, process.dv_pubkey);
+                
+            var s := map a |
+                    && a in block.body.attestations
+                    && isMyAttestation(a, process, block, valIndex)
+                ::
+                    a.data.slot := a.data;
+
+            var att_consensus_instances_already_decided := process.future_att_consensus_instances_already_decided + s;
+
+            process.(
+                    attestation_consensus_engine_state := stopConsensusInstances(
+                                    process.attestation_consensus_engine_state,
+                                    att_consensus_instances_already_decided.Keys
+                    ),
+                    attestation_shares_to_broadcast := process.attestation_shares_to_broadcast - att_consensus_instances_already_decided.Keys,
+                    rcvd_attestation_shares := process.rcvd_attestation_shares - att_consensus_instances_already_decided.Keys 
+            )      
+
+        }   
+
+        function f_listen_for_new_imported_blocks_part_3(
+            process: DVCNodeState,
+            block: BeaconBlock
+        ): DVCNodeState
+        requires f_listen_for_new_imported_blocks.requires(process, block)        
+        {
+            var valIndex := bn_get_validator_index(process.bn, block.body.state_root, process.dv_pubkey);
+                
+            var s := map a |
+                    && a in block.body.attestations
+                    && isMyAttestation(a, process, block, valIndex)
+                ::
+                    a.data.slot := a.data;
+
+            var att_consensus_instances_already_decided := process.future_att_consensus_instances_already_decided + s;
+
+            var new_future_att_consensus_instances_already_decided := 
+                    if process.latest_attestation_duty.isPresent() then
+                        var old_instances := 
+                                set i | 
+                                    && i in att_consensus_instances_already_decided.Keys
+                                    && i <= process.latest_attestation_duty.safe_get().slot
+                                ;
+                        att_consensus_instances_already_decided - old_instances
+                    else
+                        att_consensus_instances_already_decided
+                        ;
+
+            process.(
+                    future_att_consensus_instances_already_decided := new_future_att_consensus_instances_already_decided,
+                    attestation_consensus_engine_state := stopConsensusInstances(
+                                    process.attestation_consensus_engine_state,
+                                    att_consensus_instances_already_decided.Keys
+                    ),
+                    attestation_shares_to_broadcast := process.attestation_shares_to_broadcast - att_consensus_instances_already_decided.Keys,
+                    rcvd_attestation_shares := process.rcvd_attestation_shares - att_consensus_instances_already_decided.Keys 
+            )      
+        }    
+
+        function f_listen_for_new_imported_blocks_part_4(
+            process: DVCNodeState,
+            block: BeaconBlock
+        ): DVCNodeState
+        requires f_listen_for_new_imported_blocks.requires(process, block)        
+        requires 
+            var att_consensus_instances_already_decided := process.future_att_consensus_instances_already_decided + f_listen_for_new_imported_blocks_part_1(process, block);
+        
+        process.current_attesation_duty.isPresent() && process.current_attesation_duty.safe_get().slot in att_consensus_instances_already_decided        
+        {
+            var valIndex := bn_get_validator_index(process.bn, block.body.state_root, process.dv_pubkey);
+                
+            var s := map a |
+                    && a in block.body.attestations
+                    && isMyAttestation(a, process, block, valIndex)
+                ::
+                    a.data.slot := a.data;
+
+            var att_consensus_instances_already_decided := process.future_att_consensus_instances_already_decided + s;
+
+            var new_future_att_consensus_instances_already_decided := 
+                    if process.latest_attestation_duty.isPresent() then
+                        var old_instances := 
+                                set i | 
+                                    && i in att_consensus_instances_already_decided.Keys
+                                    && i <= process.latest_attestation_duty.safe_get().slot
+                                ;
+                        att_consensus_instances_already_decided - old_instances
+                    else
+                        att_consensus_instances_already_decided
+                        ;
+
+
+            var attestation_consensus_engine_state_after_stop := stopConsensusInstances(
+                                    process.attestation_consensus_engine_state,
+                                    att_consensus_instances_already_decided.Keys
+                    );    
+
+            var decided_attestation_data := att_consensus_instances_already_decided[process.current_attesation_duty.safe_get().slot];
+            var new_attestation_slashing_db := f_update_attestation_slashing_db(process.attestation_slashing_db, decided_attestation_data);                            
+
+            process.(
+                    future_att_consensus_instances_already_decided := new_future_att_consensus_instances_already_decided,
+                    attestation_shares_to_broadcast := process.attestation_shares_to_broadcast - att_consensus_instances_already_decided.Keys,
+                    rcvd_attestation_shares := process.rcvd_attestation_shares - att_consensus_instances_already_decided.Keys,
+                    current_attesation_duty := None,
+                    attestation_slashing_db := new_attestation_slashing_db,
+                    attestation_consensus_engine_state := updateConsensusInstanceValidityCheck(
+                        attestation_consensus_engine_state_after_stop,
+                        new_attestation_slashing_db
+                    )                  
+            )      
+        }                   
+      
+        function f_listen_for_new_imported_blocks_part_3_calc_old_instances(
+            att_consensus_instances_already_decided: map<Slot, AttestationData>
+        ): set<Slot>
+        requires toDVCNodeState().latest_attestation_duty.isPresent()
+        reads toDVCNodeState.reads
+        {
+            set i | 
+                && i in att_consensus_instances_already_decided.Keys
+                && i <= toDVCNodeState().latest_attestation_duty.safe_get().slot
+                              
+        }        
+
+        twostate lemma lemma_listen_for_new_imported_blocks_from_part_2_to_3_latest_attestation_duty_present(
+            p0: DVCNodeState,
+            att_consensus_instances_already_decided: map<Slot, AttestationData>,
+            old_instances: set<Slot>,
+            block: BeaconBlock
+        )      
+        requires&& (old(isValidReprExtended()) && f_listen_for_new_imported_blocks.requires(old(toDVCNodeState()), block)) 
+                && old(latest_attestation_duty).isPresent()
+                && latest_attestation_duty.isPresent()
+                && p0 == f_listen_for_new_imported_blocks_part_2(old(toDVCNodeState()), block) 
+            
+                && att_consensus_instances_already_decided == old(toDVCNodeState()).future_att_consensus_instances_already_decided + f_listen_for_new_imported_blocks_part_1(old(toDVCNodeState()), block)
+
+                && old_instances == f_listen_for_new_imported_blocks_part_3_calc_old_instances(att_consensus_instances_already_decided)
+                && toDVCNodeState() == p0.(
+                        future_att_consensus_instances_already_decided := att_consensus_instances_already_decided - old_instances
+                    )
+        ensures
+                toDVCNodeState() == f_listen_for_new_imported_blocks_part_3(old(toDVCNodeState()), block);  
+        {
+            
+        }    
+
+        twostate lemma lemma_listen_for_new_imported_blocks_from_part_2_to_3_latest_attestation_duty_not_present(
+            p0: DVCNodeState,
+            att_consensus_instances_already_decided: map<Slot, AttestationData>,
+            block: BeaconBlock
+        )      
+        requires&& (old(isValidReprExtended()) && f_listen_for_new_imported_blocks.requires(old(toDVCNodeState()), block)) 
+                && !old(latest_attestation_duty).isPresent()
+                && p0 == f_listen_for_new_imported_blocks_part_2(old(toDVCNodeState()), block) 
+            
+                && att_consensus_instances_already_decided == old(toDVCNodeState()).future_att_consensus_instances_already_decided + f_listen_for_new_imported_blocks_part_1(old(toDVCNodeState()), block)
+
+                && toDVCNodeState() == p0.(
+                        future_att_consensus_instances_already_decided := att_consensus_instances_already_decided 
+                    )
+        ensures
+                toDVCNodeState() == f_listen_for_new_imported_blocks_part_3(old(toDVCNodeState()), block);  
+        {
+            
+        }         
+
+        twostate lemma lemma_listen_for_new_imported_blocks_from_part_3_to_4(
+            p0: DVCNodeState,
+            block: BeaconBlock
+        )      
+        requires&& (old(isValidReprExtended()) && f_listen_for_new_imported_blocks.requires(old(toDVCNodeState()), block)) 
+                && p0 == f_listen_for_new_imported_blocks_part_3(old(toDVCNodeState()), block) 
+                && 
+                    var att_consensus_instances_already_decided := old(toDVCNodeState()).future_att_consensus_instances_already_decided + f_listen_for_new_imported_blocks_part_1(old(toDVCNodeState()), block);
+                &&         old(toDVCNodeState()).current_attesation_duty.isPresent() && old(toDVCNodeState()).current_attesation_duty.safe_get().slot in att_consensus_instances_already_decided 
+                &&
+                    var decided_attestation_data := att_consensus_instances_already_decided[old(toDVCNodeState()).current_attesation_duty.safe_get().slot];
+                    var new_attestation_slashing_db := f_update_attestation_slashing_db(old(toDVCNodeState()).attestation_slashing_db, decided_attestation_data); 
+                && toDVCNodeState() == p0.(
+                        current_attesation_duty := None,
+                        attestation_slashing_db := new_attestation_slashing_db,
+                        attestation_consensus_engine_state := updateConsensusInstanceValidityCheck(
+                            p0.attestation_consensus_engine_state,
+                            new_attestation_slashing_db
+                        )                             
+                    )
+        ensures
+                toDVCNodeState() == f_listen_for_new_imported_blocks_part_4(old(toDVCNodeState()), block);  
+        {
+            
+        }      
+
+        twostate predicate lemma_listen_for_new_imported_blocks_from_part_4_to_full_current_attestation_duty_has_already_been_decided_precondition(
+            p0: DVCNodeState,
+            att_consensus_instances_already_decided: map<Slot, AttestationData>,
+            block: BeaconBlock
+        )      
+        reads toDVCNodeState.reads
+        { 
+            && (old(isValidReprExtended()) && f_listen_for_new_imported_blocks.requires(old(toDVCNodeState()), block)) 
+            && old(current_attesation_duty).isPresent()
+            && p_listen_for_new_imported_blocks_part_2(old(toDVCNodeState()), block, att_consensus_instances_already_decided)
+            && old(current_attesation_duty).safe_get().slot in att_consensus_instances_already_decided
+            && p0 == f_listen_for_new_imported_blocks_part_4(old(toDVCNodeState()), block) 
+            && f_check_for_next_queued_duty.requires(p0)
+
+            && toDVCNodeState() == f_check_for_next_queued_duty(p0).state
         }
 
-        method att_consensus_decided...
-        ensures old(this.current_attesation_duty).isPresent() ==> f_att_consensus_decided(old(toDVCNodeState(this)), id, decided_attestation_data) == toDVCNodeStateAndOuputs(this);
+        twostate lemma lemma_listen_for_new_imported_blocks_from_part_4_to_full_current_attestation_duty_has_already_been_decided(
+            p0: DVCNodeState,
+            att_consensus_instances_already_decided: map<Slot, AttestationData>,
+            block: BeaconBlock
+        )      
+        requires lemma_listen_for_new_imported_blocks_from_part_4_to_full_current_attestation_duty_has_already_been_decided_precondition(p0, att_consensus_instances_already_decided, block)
+        ensures
+                toDVCNodeState()  == f_listen_for_new_imported_blocks(old(toDVCNodeState()), block).state;
         {
-            ...;
-            if old(this.current_attesation_duty).isPresent()
+            var process := old(toDVCNodeState());
+            var valIndex := bn_get_validator_index(process.bn, block.body.state_root, process.dv_pubkey);
+            
+            var s := map a |
+                    && a in block.body.attestations
+                    && isMyAttestation(a, process, block, valIndex)
+                ::
+                    a.data.slot := a.data;
+
+            var att_consensus_instances_already_decided_let := process.future_att_consensus_instances_already_decided + s;
+
+            assert att_consensus_instances_already_decided_let == old(toDVCNodeState()).future_att_consensus_instances_already_decided + f_listen_for_new_imported_blocks_part_1(old(toDVCNodeState()), block);
+
+            var future_att_consensus_instances_already_decided := 
+                    if process.latest_attestation_duty.isPresent() then
+                        var old_instances := 
+                                set i | 
+                                    && i in att_consensus_instances_already_decided_let.Keys
+                                    && i <= process.latest_attestation_duty.safe_get().slot
+                                ;
+                        att_consensus_instances_already_decided_let - old_instances
+                    else
+                        att_consensus_instances_already_decided_let
+                            ;
+
+            var newProcess :=
+                    process.(
+                        future_att_consensus_instances_already_decided := future_att_consensus_instances_already_decided,
+                        attestation_consensus_engine_state := stopConsensusInstances(
+                                        process.attestation_consensus_engine_state,
+                                        att_consensus_instances_already_decided_let.Keys
+                        ),
+                        attestation_shares_to_broadcast := process.attestation_shares_to_broadcast - att_consensus_instances_already_decided_let.Keys,
+                        rcvd_attestation_shares := process.rcvd_attestation_shares - att_consensus_instances_already_decided_let.Keys                    
+                    );    
+
+            var decided_attestation_data := att_consensus_instances_already_decided[process.current_attesation_duty.safe_get().slot];
+            var new_attestation_slashing_db := f_update_attestation_slashing_db(process.attestation_slashing_db, decided_attestation_data);
+            var newProces2 := newProcess.(
+                current_attesation_duty := None,
+                attestation_slashing_db := new_attestation_slashing_db,
+                attestation_consensus_engine_state := updateConsensusInstanceValidityCheck(
+                    newProcess.attestation_consensus_engine_state,
+                    new_attestation_slashing_db
+                )                
+            );
+            var r := f_check_for_next_queued_duty(newProces2);
+            assert newProcess.current_attesation_duty ==  process.current_attesation_duty;       
+
+            assert p0 == newProces2;   
+            assert newProcess.current_attesation_duty.isPresent() && newProcess.current_attesation_duty.safe_get().slot in att_consensus_instances_already_decided_let ;
+            assert att_consensus_instances_already_decided_let == att_consensus_instances_already_decided;
+
+            assert || f_check_for_next_queued_duty(newProces2) == f_listen_for_new_imported_blocks(process, block) 
+            by 
             {
-                assert f_att_consensus_decided(old(toDVCNodeState(this)), id, decided_attestation_data) == toDVCNodeStateAndOuputs(this);
+                assert forall a, b :: a == b &&  (f_check_for_next_queued_duty.requires(a) ||  f_check_for_next_queued_duty.requires(b)) ==> f_check_for_next_queued_duty(a) == f_check_for_next_queued_duty(b);
+            }
+                  
+        }             
+        
+
+        twostate lemma lemma_listen_for_new_imported_blocks_from_part_3_to_full_current_attestation_duty_has_not_already_been_decided(
+            block: BeaconBlock,
+            att_consensus_instances_already_decided: map<Slot, AttestationData>
+        )      
+        requires&& (old(isValidReprExtended()) && f_listen_for_new_imported_blocks.requires(old(toDVCNodeState()), block)) 
+                && att_consensus_instances_already_decided == old(toDVCNodeState()).future_att_consensus_instances_already_decided + f_listen_for_new_imported_blocks_part_1(old(toDVCNodeState()), block)
+                && 
+                    (
+                        || !old(current_attesation_duty).isPresent()
+                        || old(current_attesation_duty).safe_get().slot !in att_consensus_instances_already_decided
+                    )
+                && toDVCNodeState() == f_listen_for_new_imported_blocks_part_3(old(toDVCNodeState()), block) 
+        ensures
+                toDVCNodeState()  == f_listen_for_new_imported_blocks(old(toDVCNodeState()), block).state;
+        {
+                              
+        }                 
+
+        lemma f_listen_for_new_imported_blocks_empty_outputs(
+            process: DVCNodeState,
+            block: BeaconBlock
+        )
+        requires f_listen_for_new_imported_blocks.requires(process, block)
+        ensures f_listen_for_new_imported_blocks(process, block).outputs == getEmptyOuputs()
+        {
+            forall p | f_check_for_next_queued_duty.requires(p)
+            ensures f_check_for_next_queued_duty(p).outputs == getEmptyOuputs()
+            {
+                f_check_for_next_queued_duty_empty_outputs(p);
             }
         }
 
-        method listen_for_attestation_shares...
-        ensures f_listen_for_attestation_shares(old(toDVCNodeState(this)), attestation_share) == toDVCNodeStateAndOuputs(this);
-        {
-            ...;
-        }
 
-        // Helper function used when proving the postcondition of method listen_for_new_imported_blocks below
-        function listen_for_new_imported_blocks_helper(
-            process: DVCNodeState,
-            block: BeaconBlock,
-            valIndex: Optional<ValidatorIndex>,
-            i: nat
-        ) : (new_att: set<Slot>)
-        requires i <= |block.body.attestations|
-        requires block.body.state_root in process.bn.state_roots_of_imported_blocks
-        {            
-            set a |
-                    && a in block.body.attestations[..i]
-                    && isMyAttestation(a, process, block, valIndex)
-                ::
-                    a.data.slot
-        }           
-
-        method listen_for_new_imported_blocks...
-        ensures block.body.state_root in bn.state_roots_of_imported_blocks ==> f_listen_for_new_imported_blocks(old(toDVCNodeState(this)), block) == toDVCNodeStateAndOuputs(this);
+        lemma f_check_for_next_queued_duty_empty_outputs(
+            process: DVCNodeState
+        )
+        requires f_check_for_next_queued_duty.requires(process)
+        decreases process.attestation_duties_queue
+        ensures f_check_for_next_queued_duty(process).outputs == getEmptyOuputs()
         {
+            if  && process.attestation_duties_queue != [] 
+                && (
+                    || process.attestation_duties_queue[0].slot in process.future_att_consensus_instances_already_decided
+                    || !process.current_attesation_duty.isPresent()
+                )    
+            {
+                
+                    if process.attestation_duties_queue[0].slot in process.future_att_consensus_instances_already_decided.Keys 
+                    {
+                        var queue_head := process.attestation_duties_queue[0];
+                        var new_attestation_slashing_db := f_update_attestation_slashing_db(process.attestation_slashing_db, process.future_att_consensus_instances_already_decided[queue_head.slot]);
+                        f_check_for_next_queued_duty_empty_outputs(process.(
+                            attestation_duties_queue := process.attestation_duties_queue[1..],
+                            attestation_slashing_db := new_attestation_slashing_db,
+                            attestation_consensus_engine_state := updateConsensusInstanceValidityCheck(
+                                process.attestation_consensus_engine_state,
+                                new_attestation_slashing_db
+                            )                        
+                        ));
+                        assert f_check_for_next_queued_duty(process).outputs == getEmptyOuputs();       
+                    }
+                    else
+                    {
+                        var new_process := process.(
+                            attestation_duties_queue := process.attestation_duties_queue[1..]
+                        );  
+                        assert f_check_for_next_queued_duty(process).outputs == getEmptyOuputs();       
+                    }
+            }
+                    
+            else 
+            {
+                assert f_check_for_next_queued_duty(process).outputs == getEmptyOuputs();
+            }
+         
+        }     
+
+        twostate lemma lemaUnchangedThatImpliesEmptyOutputs()
+        requires
+            && unchanged(network`att_shares_sent)
+            && unchanged(bn`attestations_submitted)
+        ensures toDVCNodeStateAndOuputs().outputs == getEmptyOuputs()
+        {
+
+        }        
+
+        // Now that a bunch of {:fuel xxx, 0, 0} attributes have been added to listen_for_new_imported_blocks, this lemma does not seem tob be required anymore. Leaving it here, with its own old comment, just in case.
+        // 
+        // As the name of the lemma suggests, this is an unused lemma which, however, if commented out, very very very
+        // surprisingly, causes the verification time of the method listen_for_new_imported_blocks to increase to more
+        // than 30 min. lemma
+        // unused_lemma_that_if_commented_out_gets_the_verification_time_of_the_following_method_to_increase_to_30_plus_min(
+        // process: DVCNodeState, block: BeaconBlock
+        // )
+        // requires f_listen_for_new_imported_blocks.requires(process, block)  
+        // requires process.latest_attestation_duty.isPresent()                   
+        // ensures  f_listen_for_new_imported_blocks_part_3.requires(process, block) ensures  var
+        // att_consensus_instances_already_decided := process.future_att_consensus_instances_already_decided +
+        // f_listen_for_new_imported_blocks_part_1(process, block); var old_instances := set i | && i in
+        // att_consensus_instances_already_decided.Keys && i <= process.latest_attestation_duty.safe_get().slot
+        //                 ;                
+        // f_listen_for_new_imported_blocks_part_3(process, block).future_att_consensus_instances_already_decided ==
+        // att_consensus_instances_already_decided - old_instances
+        // {
+            
+        // }            
+
+        // 6min - 3.7.1
+        method  
+        {:fuel f_check_for_next_queued_duty, 0, 0} 
+        {:fuel f_update_attestation_slashing_db, 0, 0} 
+        {:fuel f_listen_for_new_imported_blocks_part_3, 0, 0}
+        {:fuel f_listen_for_new_imported_blocks_part_4, 0, 0}
+        {:fuel f_listen_for_new_imported_blocks, 0, 0}
+        listen_for_new_imported_blocks...
+        ensures (old(isValidReprExtended()) && f_listen_for_new_imported_blocks.requires(old(toDVCNodeState()), block)) ==> 
+                    && isValidReprExtended()
+                    && s.Success?
+                    && f_listen_for_new_imported_blocks(old(toDVCNodeState()), block) == toDVCNodeStateAndOuputs()
+        {
+            assert (old(isValidReprExtended()) && f_listen_for_new_imported_blocks.requires(old(toDVCNodeState()), block)) ==> block.body.state_root in bn.state_roots_of_imported_blocks;
             ...;
             while...
                 invariant 0 <= i <= |block.body.attestations|
-                invariant  block.body.state_root in old(bn.state_roots_of_imported_blocks) ==>
-                    future_att_consensus_instances_already_decided == 
-                    old(future_att_consensus_instances_already_decided) + listen_for_new_imported_blocks_helper(old(toDVCNodeState(this)), block, valIndex, i); 
+                invariant ValidRepr() && fresh(bn.Repr - old(bn.Repr)) 
+            && unchanged(rs)
+            && unchanged(network)
+            && unchanged(att_consensus)
+            && unchanged(att_consensus.consensus_instances_started.Values)
+            && unchanged(this)
+            && unchanged(att_consensus.Repr)
+            && unchanged(bn`state_roots_of_imported_blocks)
+            && unchanged(bn`attestations_submitted)
+                invariant  old(isValidReprExtended()) ==> isValidReprExtended();       
+                invariant old(isValidReprExtended()) ==> lemmaConsensusInstancesAreTheSamePrecond(att_consensus)       
+                invariant old(isValidReprExtended() )==> toDVCNodeState() == old(toDVCNodeState()) 
+                invariant unchanged(bn`attestations_submitted)
+                invariant this as object != att_consensus
+                invariant this !in att_consensus.Repr
+
+                invariant (old(isValidReprExtended()) && f_listen_for_new_imported_blocks.requires(old(toDVCNodeState()), block)) ==> p_listen_for_new_imported_blocks_part_2_for_loop_inv(old(toDVCNodeState()), block, i, att_consensus_instances_already_decided)                
+            {
+                var ax := att_consensus_instances_already_decided;
+                ...;
+                if...
+                {
+                    ...;
                     
-                invariant toDVCNodeState(this) == old(toDVCNodeState(this)).(
-                    future_att_consensus_instances_already_decided := toDVCNodeState(this).future_att_consensus_instances_already_decided
-                )
-                invariant toDVCNodeStateAndOuputs(this).outputs == getEmptyOuputs();            
+               
+
+                }
+                if (old(isValidReprExtended()) && f_listen_for_new_imported_blocks.requires(old(toDVCNodeState()), block)){
+                    lemma_f_listen_for_new_imported_blocks_part_1_to_2_for_loop_inv(old(toDVCNodeState()), block, i, ax, att_consensus_instances_already_decided);
+                }
+
+                ...;    
+            }
+            assert (old(isValidReprExtended()) && f_listen_for_new_imported_blocks.requires(old(toDVCNodeState()), block)) ==>
+                && p_listen_for_new_imported_blocks_part_2(old(toDVCNodeState()), block, att_consensus_instances_already_decided)
+                by
+            {
+                if (old(isValidReprExtended()) && f_listen_for_new_imported_blocks.requires(old(toDVCNodeState()), block)){
+                        assert isValidReprExtended();   
+                        assert lemmaConsensusInstancesAreTheSamePrecond(att_consensus);                
+                        lemma_p_listen_for_new_imported_blocks_part_2_for_loop_inv_to_part_2(old(toDVCNodeState()), block, att_consensus_instances_already_decided);
+                }   
+            }       
+ 
+            ...;
+
+            if...
             {
 
+                
+                var o1 := toDVCNodeState();
+                label L2:
+                assert (old(isValidReprExtended()) && f_listen_for_new_imported_blocks.requires(old(toDVCNodeState()), block)) ==> 
+                    && o1 == f_listen_for_new_imported_blocks_part_2(old(toDVCNodeState()), block) 
+                    && isValidReprExtended()
+                    && f_check_for_next_queued_duty.requires(toDVCNodeState())
+                    && unchanged(`current_attesation_duty)
+                    && p_listen_for_new_imported_blocks_part_2(old(toDVCNodeState()), block, att_consensus_instances_already_decided)
+                by
+                {
+                    if  (old(isValidReprExtended()) && f_listen_for_new_imported_blocks.requires(old(toDVCNodeState()), block))
+                    {
+                        assert isValidReprExtended();
+                        assert lemmaConsensusInstancesHaveBeenRemovedPrecond(att_consensus, att_consensus_instances_already_decided.Keys);
+                        lemmaConsensusInstancesHaveBeenRemoved(att_consensus, att_consensus_instances_already_decided.Keys);
+
+                        assert f_listen_for_new_imported_blocks_part_2(old(toDVCNodeState()), block).attestation_consensus_engine_state.attestation_consensus_active_instances == old(toDVCNodeState()).attestation_consensus_engine_state.attestation_consensus_active_instances - att_consensus_instances_already_decided.Keys;
+
+                        calc {
+                            o1;
+                            { lemmaConsensusInstancesAreTheSame@L2(att_consensus);}
+                            toDVCNodeState();
+                            f_listen_for_new_imported_blocks_part_2(old(toDVCNodeState()), block);        
+                        }
+
+                        assert o1 == f_listen_for_new_imported_blocks_part_2(old(toDVCNodeState()), block);   
+
+                        assert unchanged(`current_attesation_duty);                                                
+                    }
+                }
+                
+                
+                ...;
+                var o2 := toDVCNodeState();        
+                assert (old(isValidReprExtended()) && f_listen_for_new_imported_blocks.requires(old(toDVCNodeState()), block)) ==>  
+                    && o2 == f_listen_for_new_imported_blocks_part_3(old(toDVCNodeState()), block)
+                    && isValidReprExtended()  
+                    && f_check_for_next_queued_duty.requires(toDVCNodeState())
+                    && unchanged(`current_attesation_duty)
+                    && p_listen_for_new_imported_blocks_part_2(old(toDVCNodeState()), block, att_consensus_instances_already_decided)
+                by
+                {
+                    if  (old(isValidReprExtended()) && f_listen_for_new_imported_blocks.requires(old(toDVCNodeState()), block))
+                    {
+                        lemmaConsensusInstancesAreTheSame@L2(att_consensus);
+                        assert o2 == o1.(
+                            future_att_consensus_instances_already_decided := att_consensus_instances_already_decided - old_instances
+                        );
+                        lemma_listen_for_new_imported_blocks_from_part_2_to_3_latest_attestation_duty_present(o1, att_consensus_instances_already_decided, old_instances, block);
+                        assert unchanged(`current_attesation_duty);                                                   
+                    }  
+                } 
             }
+            else
+            {
+                var o1 := toDVCNodeState();
+                label L2:
+                assert (old(isValidReprExtended()) && f_listen_for_new_imported_blocks.requires(old(toDVCNodeState()), block)) ==> 
+                        && o1 == f_listen_for_new_imported_blocks_part_2(old(toDVCNodeState()), block) 
+                        && isValidReprExtended()
+                        && f_check_for_next_queued_duty.requires(toDVCNodeState())
+                        && unchanged(`current_attesation_duty)
+                        && p_listen_for_new_imported_blocks_part_2(old(toDVCNodeState()), block, att_consensus_instances_already_decided)
+                by
+                {
+                    if  (old(isValidReprExtended()) && f_listen_for_new_imported_blocks.requires(old(toDVCNodeState()), block))
+                    {
+                        assert isValidReprExtended();
+                        assert lemmaConsensusInstancesHaveBeenRemovedPrecond(att_consensus, att_consensus_instances_already_decided.Keys);
+                        lemmaConsensusInstancesHaveBeenRemoved(att_consensus, att_consensus_instances_already_decided.Keys);
+
+                        assert f_listen_for_new_imported_blocks_part_2(old(toDVCNodeState()), block).attestation_consensus_engine_state.attestation_consensus_active_instances == old(toDVCNodeState()).attestation_consensus_engine_state.attestation_consensus_active_instances - att_consensus_instances_already_decided.Keys;
+
+                        calc {
+                            o1;
+                            { lemmaConsensusInstancesAreTheSame@L2(att_consensus);}
+                            toDVCNodeState();
+                            f_listen_for_new_imported_blocks_part_2(old(toDVCNodeState()), block);        
+                        }
+
+                        assert o1 == f_listen_for_new_imported_blocks_part_2(old(toDVCNodeState()), block);            
+                        assert unchanged(`current_attesation_duty);                                        
+                    }
+                }
+                ...;
+
+                var o2 := toDVCNodeState();        
+                assert (old(isValidReprExtended()) && f_listen_for_new_imported_blocks.requires(old(toDVCNodeState()), block)) ==>  
+                    && o2 == f_listen_for_new_imported_blocks_part_3(old(toDVCNodeState()), block)  
+                    && isValidReprExtended()
+                    && f_check_for_next_queued_duty.requires(toDVCNodeState())
+                    && unchanged(`current_attesation_duty)
+                    && p_listen_for_new_imported_blocks_part_2(old(toDVCNodeState()), block, att_consensus_instances_already_decided)
+                by
+                {
+                    if  (old(isValidReprExtended()) && f_listen_for_new_imported_blocks.requires(old(toDVCNodeState()), block))
+                    {
+                        assert isValidReprExtended();   
+
+                        var o2 := toDVCNodeState();
+                        lemmaConsensusInstancesAreTheSame@L2(att_consensus);
+                        assert o2 == o1.(
+                            future_att_consensus_instances_already_decided := att_consensus_instances_already_decided 
+                        );
+                        lemma_listen_for_new_imported_blocks_from_part_2_to_3_latest_attestation_duty_not_present(o1, att_consensus_instances_already_decided, block);
+                        assert unchanged(`current_attesation_duty);                                                                    
+                    } 
+                }                                         
+            }     
+
+            if...
+            {
+                label L3:
+                var o3 := toDVCNodeState();
+                assert (old(isValidReprExtended()) && f_listen_for_new_imported_blocks.requires(old(toDVCNodeState()), block)) ==>  
+                    && toDVCNodeState() == f_listen_for_new_imported_blocks_part_3(old(toDVCNodeState()), block)
+                    && isValidReprExtended()
+                    && f_check_for_next_queued_duty.requires(toDVCNodeState())
+                    && unchanged(`current_attesation_duty)
+                    && p_listen_for_new_imported_blocks_part_2(old(toDVCNodeState()), block, att_consensus_instances_already_decided)
+                    && old(current_attesation_duty).safe_get().slot in att_consensus_instances_already_decided
+                    ;
+                
+                ...;
+                {
+                    var o4 := toDVCNodeState();
+                    assert (old(isValidReprExtended()) && f_listen_for_new_imported_blocks.requires(old(toDVCNodeState()), block)) ==>  
+                        && o4 == f_listen_for_new_imported_blocks_part_4(old(toDVCNodeState()), block)
+                        && isValidReprExtended()
+                        && f_check_for_next_queued_duty.requires(toDVCNodeState())
+                        && old(current_attesation_duty).safe_get().slot in att_consensus_instances_already_decided
+                        && p_listen_for_new_imported_blocks_part_2(old(toDVCNodeState()), block, att_consensus_instances_already_decided)
+                    by 
+                    {
+                        if  (old(isValidReprExtended()) && f_listen_for_new_imported_blocks.requires(old(toDVCNodeState()), block))
+                        {
+                            lemmaAttestationHasBeenAddedToSlashingDbForall@L3(att_consensus_instances_already_decided[old@L3(current_attesation_duty).safe_get().slot]);
+                            lemma_listen_for_new_imported_blocks_from_part_3_to_4(o3, block);
+                            assert o4 == f_listen_for_new_imported_blocks_part_4(old(toDVCNodeState()), block);  
+                        }
+                    } 
+                    
+                    ...;
+                    assert (old(isValidReprExtended()) && f_listen_for_new_imported_blocks.requires(old(toDVCNodeState()), block)) ==>  toDVCNodeState() == f_listen_for_new_imported_blocks(old(toDVCNodeState()), block).state by       
+                    {
+                        if  (old(isValidReprExtended()) && f_listen_for_new_imported_blocks.requires(old(toDVCNodeState()), block))
+                        {
+                            assert lemma_listen_for_new_imported_blocks_from_part_4_to_full_current_attestation_duty_has_already_been_decided_precondition(o4, att_consensus_instances_already_decided, block) by 
+                            {
+                                assert 
+                                && p_listen_for_new_imported_blocks_part_2(old(toDVCNodeState()), block, att_consensus_instances_already_decided)
+                                && old(current_attesation_duty).safe_get().slot in att_consensus_instances_already_decided
+                                && o4 == f_listen_for_new_imported_blocks_part_4(old(toDVCNodeState()), block) 
+                                && f_check_for_next_queued_duty.requires(o4)
+                                && toDVCNodeState() == f_check_for_next_queued_duty(o4).state
+                                ;                                
+                            }    
+
+                            lemma_listen_for_new_imported_blocks_from_part_4_to_full_current_attestation_duty_has_already_been_decided(o4, att_consensus_instances_already_decided, block);  
+                        }
+                    }                                   
+
+                }
+            }
+            else
+            {
+                var o3 := toDVCNodeState();
+                assert (old(isValidReprExtended()) && f_listen_for_new_imported_blocks.requires(old(toDVCNodeState()), block)) ==>  
+                    && toDVCNodeState() == f_listen_for_new_imported_blocks_part_3(old(toDVCNodeState()), block)
+                    && isValidReprExtended()
+                    && f_check_for_next_queued_duty.requires(toDVCNodeState())
+                    && unchanged(`current_attesation_duty)
+                    ;
+                if  (old(isValidReprExtended()) && f_listen_for_new_imported_blocks.requires(old(toDVCNodeState()), block))
+                {
+                    // assert !old(current_attesation_duty).isPresent();
+                    lemma_listen_for_new_imported_blocks_from_part_3_to_full_current_attestation_duty_has_not_already_been_decided(block, att_consensus_instances_already_decided);
+                }
+            }
+            if  (old(isValidReprExtended()) && f_listen_for_new_imported_blocks.requires(old(toDVCNodeState()), block))
+            {
+                assert toDVCNodeState() == f_listen_for_new_imported_blocks(old(toDVCNodeState()), block).state;  
+                assert unchanged(network);
+                assert unchanged(bn`attestations_submitted);
+                lemaUnchangedThatImpliesEmptyOutputs();
+                f_listen_for_new_imported_blocks_empty_outputs(old(toDVCNodeState()), block);               
+            }            
+            ...;
         }
 
         method resend_attestation_share...
-        ensures f_resend_attestation_share(old(toDVCNodeState(this))) == toDVCNodeStateAndOuputs(this)
+        ensures old(isValidReprExtended()) ==>
+                                && isValidReprExtended()
+                                && f_resend_attestation_share(old(toDVCNodeState())) == toDVCNodeStateAndOuputs()
         {
             ...;
-            assert  f_resend_attestation_share(old(toDVCNodeState(this))) == toDVCNodeStateAndOuputs(this);
+            assert  old(isValidReprExtended()) ==> f_resend_attestation_share(old(toDVCNodeState())).state == toDVCNodeStateAndOuputs().state;
+            var setWithRecipient := set att_share | att_share in attestation_shares_to_broadcast.Values :: addRecepientsToMessage(att_share, peers);
+            var setWithRecipientFlattened := setUnion(setWithRecipient);
+            assert old(isValidReprExtended()) ==>network.att_shares_sent == old(network.att_shares_sent) +[setWithRecipientFlattened];                
+            assert old(isValidReprExtended()) ==>seqMinusToSet(network.att_shares_sent, old(network.att_shares_sent)) == {setWithRecipientFlattened};
+            assert  old(isValidReprExtended()) ==>toDVCNodeStateAndOuputs().outputs.att_shares_sent == setWithRecipientFlattened;
+            assert  old(isValidReprExtended()) ==>f_resend_attestation_share(old(toDVCNodeState())) == toDVCNodeStateAndOuputs();                  
         }
     }
 }
+
+// Keep this here as it does come handy from time to time
+// var o := toDVCNodeState();
+// var rs := r.state;
+
+// assert rs.attestation_consensus_engine_state == o.attestation_consensus_engine_state;
+
+// assert rs == o.(
+//     // current_attesation_duty := rs.current_attesation_duty,
+//     latest_attestation_duty := rs.latest_attestation_duty,
+//     attestation_duties_queue := rs.attestation_duties_queue,
+//     attestation_slashing_db := rs.attestation_slashing_db,
+//     rcvd_attestation_shares := rs.rcvd_attestation_shares,
+//     attestation_shares_to_broadcast := rs.attestation_shares_to_broadcast,
+//     // attestation_consensus_engine_state := rs.attestation_consensus_engine_state,
+//     // attestation_validity_check
+//     peers := rs.peers,
+//     construct_signed_attestation_signature := rs.construct_signed_attestation_signature,
+//     // TODO := rs.// TODO,
+//     dv_pubkey := rs.dv_pubkey,
+//     future_att_consensus_instances_already_decided := rs.future_att_consensus_instances_already_decided//,
+//     // bn := rs.bn//,
+//     // rs := rs.rs
+// )
+// ;  
