src/dvspec/dafny/specification/dvc_spec.dfy
@@ -2,10 +2,9 @@ include "../commons.dfy"
 include "../implementation/dvc_implementation.dfy"
 
 
-abstract module DVCNode_Spec {
+module DVCNode_Spec {
     import opened Types 
     import opened CommonFunctions
-    import opened DVCNode_Implementation`PublicInterface
     import opened DVCNode_Externs
 
     function {:axiom} bn_get_fork_version(slot: Slot): Version
@@ -51,16 +50,89 @@ abstract module DVCNode_Spec {
         state_roots_of_imported_blocks: set<Root>   
     )
 
-    function getInitialBN(): BNState
-    {
-        BNState(
-            state_roots_of_imported_blocks := {}
-        )
-    }    
+    // function getInitialBN(): BNState
+    // {
+    //     BNState(
+    //         state_roots_of_imported_blocks := {}
+    //     )
+    // }    
 
     datatype RSState = RSState(
         pubkey: BLSPubkey
     )
+
+    datatype AttestationConsensusValidityCheckState = AttestationConsensusValidityCheckState(
+        attestation_duty: AttestationDuty,
+        validityPredicate: AttestationData -> bool
+    )
+
+    datatype ConsensusEngineState = ConsensusEngineState(
+        attestation_consensus_active_instances: map<Slot, AttestationConsensusValidityCheckState>
+    )
+
+    function getInitialConensusEngineState(): ConsensusEngineState
+    {
+        ConsensusEngineState(
+            attestation_consensus_active_instances := map[]
+        )
+    }
+
+    function startConsensusInstance(
+        s: ConsensusEngineState,
+        id: Slot,
+        attestation_duty: AttestationDuty,
+        attestation_slashing_db: set<SlashingDBAttestation>
+    ): ConsensusEngineState
+    requires id !in s.attestation_consensus_active_instances.Keys
+    {
+        var acvc := AttestationConsensusValidityCheckState(
+                    attestation_duty := attestation_duty,
+                    validityPredicate := (ad: AttestationData) => consensus_is_valid_attestation_data(attestation_slashing_db, ad, attestation_duty)
+                );
+        assert (acvc.validityPredicate == (ad: AttestationData) => consensus_is_valid_attestation_data(attestation_slashing_db, ad, acvc.attestation_duty));
+        s.(
+            attestation_consensus_active_instances := s.attestation_consensus_active_instances[
+                id := acvc
+            ]
+        )
+    }
+
+    function stopConsensusInstances(
+        s: ConsensusEngineState,
+        ids: set<Slot>
+    ): ConsensusEngineState
+    {
+        s.(
+            attestation_consensus_active_instances := s.attestation_consensus_active_instances - ids
+        )
+    }    
+
+    function updateConsensusInstanceValidityCheckHelper(
+        m: map<Slot, AttestationConsensusValidityCheckState>,
+        new_attestation_slashing_db: set<SlashingDBAttestation>
+    ): (r: map<Slot, AttestationConsensusValidityCheckState>)
+    ensures r.Keys <= m.Keys
+    {
+            map it | it in m.Items
+                ::
+                it.0 := it.1.(
+                    validityPredicate := (ad: AttestationData) => consensus_is_valid_attestation_data(new_attestation_slashing_db, ad, it.1.attestation_duty)
+                )        
+    }
+
+    function updateConsensusInstanceValidityCheck(
+        s: ConsensusEngineState,
+        new_attestation_slashing_db: set<SlashingDBAttestation>
+    ): (r: ConsensusEngineState)
+    {
+        s.(
+            attestation_consensus_active_instances := 
+                updateConsensusInstanceValidityCheckHelper(
+                    s.attestation_consensus_active_instances,
+                    new_attestation_slashing_db
+                )
+        )
+    }
 
     function getInitialRS(
         pubkey: BLSPubkey
@@ -73,29 +145,29 @@ abstract module DVCNode_Spec {
 
     datatype DVCNodeState = DVCNodeState(
         current_attesation_duty: Optional<AttestationDuty>,
+        latest_attestation_duty: Optional<AttestationDuty>,
         attestation_duties_queue: seq<AttestationDuty>,
-        attestation_slashing_db: AttestationSlashingDB,
-        attestation_shares_db: AttestationSignatureShareDB,
-        attestation_share_to_broadcast: Optional<AttestationShare>,
+        attestation_slashing_db: set<SlashingDBAttestation>,
+        rcvd_attestation_shares: map<Slot,map<(AttestationData, seq<bool>), set<AttestationShare>>>,
+        attestation_shares_to_broadcast: map<Slot, AttestationShare>,
+        attestation_consensus_engine_state: ConsensusEngineState,
         peers: set<BLSPubkey>,
         construct_signed_attestation_signature: (set<AttestationShare>) -> Optional<BLSSignature>,
         // TODO: Note difference with spec.py
         dv_pubkey: BLSPubkey,
-        future_att_consensus_instances_already_decided: set<Slot>,
+        future_att_consensus_instances_already_decided:  map<Slot, AttestationData>,
         bn: BNState,
         rs: RSState
-    )    
+    )
 
     datatype Outputs = Outputs(
         att_shares_sent: set<MessaageWithRecipient<AttestationShare>>,
-        att_consensus_commands_sent: set<ConsensusCommand>,
         attestations_submitted: set<Attestation>
     )    
 
     function getEmptyOuputs(): Outputs
     {
         Outputs(
-            {},
             {},
             {}
         )
@@ -107,39 +179,40 @@ abstract module DVCNode_Spec {
         addRecepientsToMessage(m, receipients)
     }
 
+    function multicast_multiple<M>(ms: set<M>, receipients: set<BLSPubkey>): set<MessaageWithRecipient<M>>
+    {
+        var setWithRecipient := set m | m in ms :: addRecepientsToMessage(m, receipients);
+        setUnion(setWithRecipient)
+    }    
+
     datatype DVCNodeStateAndOuputs = DVCNodeStateAndOuputs(
         state: DVCNodeState,
         outputs: Outputs
     )
 
-    datatype Event = 
-    | ServeAttstationDuty(attestation_duty: AttestationDuty)
-    | AttConsensusDecided(id: Slot, decided_attestation_data: AttestationData)
-    | ReceviedAttesttionShare(attestation_share: AttestationShare)
-    | ImportedNewBlock(block: BeaconBlock)
-    | ResendAttestationShares
-    | NoEvent
-
-
     predicate Init(
         s: DVCNodeState,
         dv_pubkey: BLSPubkey,
         peers: set<BLSPubkey>,
-        construct_signed_attestation_signature: (set<AttestationShare>) -> Optional<BLSSignature>
+        construct_signed_attestation_signature: (set<AttestationShare>) -> Optional<BLSSignature>,
+        initial_attestation_slashing_db: set<SlashingDBAttestation>,
+        rs_pubkey: BLSPubkey
     )
     {
         s == DVCNodeState(
             current_attesation_duty := None,
+            latest_attestation_duty := None,
             attestation_duties_queue := [],
-            attestation_slashing_db := {},
-            attestation_shares_db := map[],
-            attestation_share_to_broadcast := None,
+            attestation_slashing_db := initial_attestation_slashing_db,
+            rcvd_attestation_shares := map[],
+            attestation_shares_to_broadcast := map[],
+            attestation_consensus_engine_state := getInitialConensusEngineState(),
             peers := peers,
             construct_signed_attestation_signature := construct_signed_attestation_signature,
             dv_pubkey := dv_pubkey,
-            future_att_consensus_instances_already_decided := {},
-            bn := getInitialBN(),
-            rs := s.rs
+            future_att_consensus_instances_already_decided := map[],
+            bn := s.bn,
+            rs := getInitialRS(rs_pubkey)
         )
     }
 
@@ -157,7 +230,8 @@ abstract module DVCNode_Spec {
 
         match event 
             case ServeAttstationDuty(attestation_duty) => 
-                f_serve_attestation_duty(s, attestation_duty) == newNodeStateAndOutputs
+                && f_serve_attestation_duty.requires(s, attestation_duty)
+                && f_serve_attestation_duty(s, attestation_duty) == newNodeStateAndOutputs
             case AttConsensusDecided(id, decided_attestation_data) => 
                 && f_att_consensus_decided.requires(s, id,  decided_attestation_data)
                 && f_att_consensus_decided(s, id,  decided_attestation_data) == newNodeStateAndOutputs
@@ -172,10 +246,45 @@ abstract module DVCNode_Spec {
                 DVCNodeStateAndOuputs(state := s, outputs := getEmptyOuputs() ) == newNodeStateAndOutputs
     }
 
+    function f_process_event(
+        s: DVCNodeState,
+        event: Event
+    ): DVCNodeStateAndOuputs
+    requires
+            match event 
+            case ServeAttstationDuty(attestation_duty) => 
+                && f_serve_attestation_duty.requires(s, attestation_duty)
+            case AttConsensusDecided(id, decided_attestation_data) => 
+                && f_att_consensus_decided.requires(s, id,  decided_attestation_data)
+            case ReceviedAttesttionShare(attestation_share) => 
+                f_listen_for_attestation_shares.requires(s, attestation_share)
+            case ImportedNewBlock(block) => 
+                f_listen_for_new_imported_blocks.requires(s, block)
+            case ResendAttestationShares => 
+                f_resend_attestation_share.requires(s) 
+            case NoEvent => 
+                true
+    {
+        match event 
+            case ServeAttstationDuty(attestation_duty) => 
+                f_serve_attestation_duty(s, attestation_duty)
+            case AttConsensusDecided(id, decided_attestation_data) => 
+                f_att_consensus_decided(s, id,  decided_attestation_data)
+            case ReceviedAttesttionShare(attestation_share) => 
+                f_listen_for_attestation_shares(s, attestation_share)
+            case ImportedNewBlock(block) => 
+                f_listen_for_new_imported_blocks(s, block)
+            case ResendAttestationShares => 
+                f_resend_attestation_share(s)
+            case NoEvent => 
+                DVCNodeStateAndOuputs(state := s, outputs := getEmptyOuputs() )
+    }    
+
     function f_serve_attestation_duty(
         process: DVCNodeState,
         attestation_duty: AttestationDuty
     ): DVCNodeStateAndOuputs
+    requires forall ad | ad in process.attestation_duties_queue + [attestation_duty]:: ad.slot !in process.attestation_consensus_engine_state.attestation_consensus_active_instances.Keys
     {
         f_check_for_next_queued_duty(
             process.(
@@ -185,16 +294,33 @@ abstract module DVCNode_Spec {
     }    
 
     function f_check_for_next_queued_duty(process: DVCNodeState): DVCNodeStateAndOuputs
+    requires forall ad | ad in process.attestation_duties_queue :: ad.slot !in process.attestation_consensus_engine_state.attestation_consensus_active_instances.Keys
     decreases process.attestation_duties_queue
     {
-        if process.attestation_duties_queue != [] then
+        if  && process.attestation_duties_queue != [] 
+            && (
+                || process.attestation_duties_queue[0].slot in process.future_att_consensus_instances_already_decided
+                || !process.current_attesation_duty.isPresent()
+            )    
+        then
             
-                if process.attestation_duties_queue[0].slot in process.future_att_consensus_instances_already_decided then
+                if process.attestation_duties_queue[0].slot in process.future_att_consensus_instances_already_decided.Keys then
+                    var queue_head := process.attestation_duties_queue[0];
+                    var new_attestation_slashing_db := f_update_attestation_slashing_db(process.attestation_slashing_db, process.future_att_consensus_instances_already_decided[queue_head.slot]);
                     f_check_for_next_queued_duty(process.(
-                        attestation_duties_queue := process.attestation_duties_queue[1..]
+                        attestation_duties_queue := process.attestation_duties_queue[1..],
+                        future_att_consensus_instances_already_decided := process.future_att_consensus_instances_already_decided - {queue_head.slot},
+                        attestation_slashing_db := new_attestation_slashing_db,
+                        attestation_consensus_engine_state := updateConsensusInstanceValidityCheck(
+                            process.attestation_consensus_engine_state,
+                            new_attestation_slashing_db
+                        )                        
                     ))
                 else
-                    f_start_next_duty(process, process.attestation_duties_queue[0])
+                    var new_process := process.(
+                        attestation_duties_queue := process.attestation_duties_queue[1..]
+                    );         
+                    f_start_next_duty(new_process, process.attestation_duties_queue[0])
                 
         else 
             DVCNodeStateAndOuputs(
@@ -205,16 +331,24 @@ abstract module DVCNode_Spec {
     }         
 
     function f_start_next_duty(process: DVCNodeState, attestation_duty: AttestationDuty): DVCNodeStateAndOuputs
+    requires attestation_duty.slot !in process.attestation_consensus_engine_state.attestation_consensus_active_instances.Keys
     {
+        var validityPredicate := 
+                (ad: AttestationData)  => 
+                    consensus_is_valid_attestation_data(process.attestation_slashing_db, ad, attestation_duty)
+                ;        
         DVCNodeStateAndOuputs(
             state :=  process.(
-                        attestation_shares_db := map[],
-                        attestation_share_to_broadcast := None,
-                        current_attesation_duty := Some(attestation_duty)
+                        current_attesation_duty := Some(attestation_duty),
+                        latest_attestation_duty := Some(attestation_duty),
+                        attestation_consensus_engine_state := startConsensusInstance(
+                            process.attestation_consensus_engine_state,
+                            attestation_duty.slot,
+                            attestation_duty,
+                            process.attestation_slashing_db
+                        )
             ),
-            outputs := getEmptyOuputs().(
-                att_consensus_commands_sent := {ConsensusCommand.Start(attestation_duty.slot)}
-            )
+            outputs := getEmptyOuputs()
         )        
     }      
 
@@ -225,15 +359,12 @@ abstract module DVCNode_Spec {
         seq(index, i => if i + 1 == index then true else false)
     } 
 
-    function f_update_attestation_slashing_db(attestation_slashing_db: AttestationSlashingDB, attestation_data: AttestationData, attestation_duty_pubkey: BLSPubkey): AttestationSlashingDB     
+    function f_update_attestation_slashing_db(attestation_slashing_db: set<SlashingDBAttestation>, attestation_data: AttestationData): set<SlashingDBAttestation>     
     {
-        // assert not is_slashable_attestation_data(attestation_slashing_db, attestation_data, pubkey)
-        // TODO: Is the following required given that each co-validator only handles one pubkey?
-        // slashing_db_data = get_slashing_db_data_for_pubkey(attestation_slashing_db, pubkey)
         var slashing_db_attestation := SlashingDBAttestation(
                                             source_epoch := attestation_data.source.epoch,
                                             target_epoch := attestation_data.target.epoch,
-                                            signing_root := hash_tree_root(attestation_data));
+                                            signing_root := Some(hash_tree_root(attestation_data)));
         
         attestation_slashing_db + {slashing_db_attestation}
     }      
@@ -244,28 +375,39 @@ abstract module DVCNode_Spec {
         decided_attestation_data: AttestationData
     ): DVCNodeStateAndOuputs
     requires process.current_attesation_duty.isPresent()
+    requires forall ad | ad in process.attestation_duties_queue :: ad.slot !in process.attestation_consensus_engine_state.attestation_consensus_active_instances.Keys    
     {
         var local_current_attestation_duty := process.current_attesation_duty.safe_get();
-        var attestation_slashing_db := f_update_attestation_slashing_db(process.attestation_slashing_db, decided_attestation_data, local_current_attestation_duty.pubkey);
+        var attestation_slashing_db := f_update_attestation_slashing_db(process.attestation_slashing_db, decided_attestation_data);
 
         var fork_version := bn_get_fork_version(compute_start_slot_at_epoch(decided_attestation_data.target.epoch));
         var attestation_signing_root := compute_attestation_signing_root(decided_attestation_data, fork_version);
         var attestation_signature_share := rs_sign_attestation(decided_attestation_data, fork_version, attestation_signing_root, process.rs);
-        // TODO: What is attestation_signature_share.aggregation_bits?
         var attestation_with_signature_share := AttestationShare(
                 aggregation_bits := get_aggregation_bits(local_current_attestation_duty.validator_index),
                 data := decided_attestation_data, 
-                signature :=attestation_signature_share
+                signature := attestation_signature_share
             ); 
 
-        DVCNodeStateAndOuputs(
-            state := process.(
-                attestation_share_to_broadcast := Some(attestation_with_signature_share)
-            ),
+        var process := 
+            process.(
+                current_attesation_duty := None,
+                attestation_shares_to_broadcast := process.attestation_shares_to_broadcast[local_current_attestation_duty.slot := attestation_with_signature_share],
+                attestation_slashing_db := attestation_slashing_db,
+                attestation_consensus_engine_state := updateConsensusInstanceValidityCheck(
+                    process.attestation_consensus_engine_state,
+                    attestation_slashing_db
+                )
+            );
+
+        var ret_check_for_next_queued_duty := f_check_for_next_queued_duty(process);
+
+        ret_check_for_next_queued_duty.(
+            state := ret_check_for_next_queued_duty.state,
             outputs := getEmptyOuputs().(
                 att_shares_sent := multicast(attestation_with_signature_share, process.peers)
-            )
-        )         
+            )          
+        )        
     }    
 
     function f_listen_for_attestation_shares(
@@ -273,37 +415,58 @@ abstract module DVCNode_Spec {
         attestation_share: AttestationShare
     ): DVCNodeStateAndOuputs
     {
-        var k := (attestation_share.data, attestation_share.aggregation_bits);
+        var activate_att_consensus_intances := process.attestation_consensus_engine_state.attestation_consensus_active_instances.Keys;
 
-        var newProcess := process.(
-            attestation_shares_db := 
-                process.attestation_shares_db[k := 
-                                        getOrDefault(process.attestation_shares_db, k, {}) + 
-                                        {attestation_share}
-                                    ]
-        );
+        if 
+            || (activate_att_consensus_intances == {} && !process.latest_attestation_duty.isPresent())
+            || (activate_att_consensus_intances != {} && minSet(activate_att_consensus_intances) <= attestation_share.data.slot)
+            || (activate_att_consensus_intances == {} && process.current_attesation_duty.isPresent() && process.current_attesation_duty.safe_get().slot <= attestation_share.data.slot)                
+            || (activate_att_consensus_intances == {} && !process.current_attesation_duty.isPresent() && process.latest_attestation_duty.isPresent() && process.latest_attestation_duty.safe_get().slot < attestation_share.data.slot) then
 
-                    
-        if process.construct_signed_attestation_signature(newProcess.attestation_shares_db[k]).isPresent() then
-        
-            var aggregated_attestation := 
-                    Attestation(
-                        aggregation_bits := attestation_share.aggregation_bits,
-                        data := attestation_share.data,
-                        signature := process.construct_signed_attestation_signature(newProcess.attestation_shares_db[k]).safe_get()
-                    );
+                var k := (attestation_share.data, attestation_share.aggregation_bits);
+                var attestation_shares_db_at_slot := getOrDefault(process.rcvd_attestation_shares, attestation_share.data.slot, map[]);
+                
+                var new_attestation_shares_db := 
+                        process.rcvd_attestation_shares[
+                            attestation_share.data.slot := 
+                                attestation_shares_db_at_slot[
+                                            k := 
+                                                getOrDefault(attestation_shares_db_at_slot, k, {}) + 
+                                                {attestation_share}
+                                            ]
+                                ];
 
+                var process := process.(
+                    rcvd_attestation_shares := new_attestation_shares_db
+                );
+
+                            
+                if process.construct_signed_attestation_signature(process.rcvd_attestation_shares[attestation_share.data.slot][k]).isPresent() then
+                
+                    var aggregated_attestation := 
+                            Attestation(
+                                aggregation_bits := attestation_share.aggregation_bits,
+                                data := attestation_share.data,
+                                signature := process.construct_signed_attestation_signature(process.rcvd_attestation_shares[attestation_share.data.slot][k]).safe_get()
+                            );
+
+                    DVCNodeStateAndOuputs(
+                        state := process,
+                        outputs := getEmptyOuputs()
+                        .(
+                            attestations_submitted := {aggregated_attestation} 
+                        )
+                    ) 
+                else 
+                    DVCNodeStateAndOuputs(
+                        state := process,
+                        outputs := getEmptyOuputs()
+                    ) 
+        else
             DVCNodeStateAndOuputs(
-                state := newProcess,
-                outputs := getEmptyOuputs().(
-                    attestations_submitted := {aggregated_attestation} 
-                )
-            ) 
-        else 
-            DVCNodeStateAndOuputs(
-                state := newProcess,
+                state := process,
                 outputs := getEmptyOuputs()
-            ) 
+            )         
     }
  
     predicate isMyAttestation(
@@ -319,8 +482,32 @@ abstract module DVCNode_Spec {
             && valIndex.v in committee
             && var i:nat :| i < |committee| && committee[i] == valIndex.v;
             && i < |a.aggregation_bits|
-            && a.aggregation_bits[i]
-            && (process.current_attesation_duty.isPresent() ==> a.data.slot >= process.current_attesation_duty.safe_get().slot)            
+            && a.aggregation_bits[i]         
+    }
+
+    function f_listen_for_new_imported_blocks_compute_att_consensus_instances_already_decided(
+        process: DVCNodeState,
+        block: BeaconBlock,
+        valIndex: Optional<ValidatorIndex>,
+        att_consensus_instances_already_decided: map<Slot, AttestationData>,
+        i: nat := 0
+    ): map<Slot, AttestationData>
+    requires i <= |block.body.attestations|
+    requires block.body.state_root in process.bn.state_roots_of_imported_blocks
+    decreases |block.body.attestations| - i
+    {
+        var attestations := block.body.attestations;
+        if |attestations| == i then 
+            att_consensus_instances_already_decided
+        else
+            var a := attestations[i];
+            var new_att_consensus_instances_already_decided := 
+                if isMyAttestation(a, process, block, valIndex) then
+                    att_consensus_instances_already_decided[a.data.slot := a.data]
+                else
+                    att_consensus_instances_already_decided
+                ;
+            f_listen_for_new_imported_blocks_compute_att_consensus_instances_already_decided( process, block, valIndex, new_att_consensus_instances_already_decided, i + 1)
     }
 
     function f_listen_for_new_imported_blocks(
@@ -328,31 +515,65 @@ abstract module DVCNode_Spec {
         block: BeaconBlock
     ): DVCNodeStateAndOuputs
     requires block.body.state_root in process.bn.state_roots_of_imported_blocks
+    requires    var valIndex := bn_get_validator_index(process.bn, block.body.state_root, process.dv_pubkey);
+                forall a1, a2 | 
+                        && a1 in block.body.attestations
+                        && isMyAttestation(a1, process, block, valIndex)
+                        && a2 in block.body.attestations
+                        && isMyAttestation(a2, process, block, valIndex)                        
+                    ::
+                        a1.data.slot == a2.data.slot ==> a1 == a2
+    requires forall ad | ad in process.attestation_duties_queue :: ad.slot !in process.attestation_consensus_engine_state.attestation_consensus_active_instances.Keys
     {
         var valIndex := bn_get_validator_index(process.bn, block.body.state_root, process.dv_pubkey);
          
-        var s := set a |
+        var s := map a |
                 && a in block.body.attestations
                 && isMyAttestation(a, process, block, valIndex)
             ::
-                a.data.slot;
+                a.data.slot := a.data;
 
-        var newProces := process.(
-            future_att_consensus_instances_already_decided := process.future_att_consensus_instances_already_decided + s
-        );
+        var att_consensus_instances_already_decided := process.future_att_consensus_instances_already_decided + s;
 
-        if process.current_attesation_duty.isPresent() && process.current_attesation_duty.safe_get().slot in process.future_att_consensus_instances_already_decided then
+        var future_att_consensus_instances_already_decided := 
+                if process.latest_attestation_duty.isPresent() then
+                    var old_instances := 
+                            set i | 
+                                && i in att_consensus_instances_already_decided.Keys
+                                && i <= process.latest_attestation_duty.safe_get().slot
+                            ;
+                    att_consensus_instances_already_decided - old_instances
+                else
+                    att_consensus_instances_already_decided
+                        ;
+
+        var process :=
+                process.(
+                    future_att_consensus_instances_already_decided := future_att_consensus_instances_already_decided,
+                    attestation_consensus_engine_state := stopConsensusInstances(
+                                    process.attestation_consensus_engine_state,
+                                    att_consensus_instances_already_decided.Keys
+                    ),
+                    attestation_shares_to_broadcast := process.attestation_shares_to_broadcast - att_consensus_instances_already_decided.Keys,
+                    rcvd_attestation_shares := process.rcvd_attestation_shares - att_consensus_instances_already_decided.Keys                    
+                );                    
+
+        if process.current_attesation_duty.isPresent() && process.current_attesation_duty.safe_get().slot in att_consensus_instances_already_decided then
             // Stop(current_attesation_duty.safe_get().slot);
-            var r := f_check_for_next_queued_duty(newProces);
-            DVCNodeStateAndOuputs(
-                state := r.state,
-                outputs := r.outputs.(
-                    att_consensus_commands_sent := r.outputs.att_consensus_commands_sent + {ConsensusCommand.Stop(process.current_attesation_duty.safe_get().slot)}
-                )
-            )
+            var decided_attestation_data := att_consensus_instances_already_decided[process.current_attesation_duty.safe_get().slot];
+            var new_attestation_slashing_db := f_update_attestation_slashing_db(process.attestation_slashing_db, decided_attestation_data);
+            var process := process.(
+                current_attesation_duty := None,
+                attestation_slashing_db := new_attestation_slashing_db,
+                attestation_consensus_engine_state := updateConsensusInstanceValidityCheck(
+                    process.attestation_consensus_engine_state,
+                    new_attestation_slashing_db
+                )                
+            );
+            f_check_for_next_queued_duty(process)
         else
             DVCNodeStateAndOuputs(
-                state := newProces,
+                state := process,
                 outputs := getEmptyOuputs()
             )
     }    
@@ -365,17 +586,14 @@ abstract module DVCNode_Spec {
             state := process,
             outputs := getEmptyOuputs().(
                 att_shares_sent :=
-                    if process.attestation_share_to_broadcast.isPresent() then
-                        multicast(process.attestation_share_to_broadcast.safe_get(), process.peers)
-                    else
-                        {}
-                    )
+                    multicast_multiple(process.attestation_shares_to_broadcast.Values, process.peers)
+            )
         )
 
     }        
 }
 
-abstract module DVCNode_Externs_Proofs refines DVCNode_Externs
+module DVCNode_Externs_Proofs refines DVCNode_Externs
 {
     import opened DVCNode_Spec
 
@@ -387,7 +605,7 @@ abstract module DVCNode_Externs_Proofs refines DVCNode_Externs
         )
     }
 
-    class BeaconNode...
+    trait BeaconNode...
     {
         method get_fork_version...
         ensures bn_get_fork_version(s) == v
@@ -400,7 +618,7 @@ abstract module DVCNode_Externs_Proofs refines DVCNode_Externs
     }
 
 
-    class RemoteSigner...
+    trait RemoteSigner...
     {
         method sign_attestation...
         ensures rs_sign_attestation(attestation_data, fork_version, signing_root, toRSState(this)) == s
